Update shift and rotate Simplicity implementions in Coq.
This update matches the definitions from Haskell that are used in jet
specifications.

In particular, the Simplicity SHA256 compression function implementation now
matches the Simplicity specification defined in Haskell.

Coq/Simplicity/SHA256.v
@@ -85,10 +85,10 @@ Definition majWord32 {term : Core.Algebra} : term (Word32 * (Word32 * Word32)) W
   bitwiseTri maj.
 
 Definition shift32 z {term : Core.Algebra} : term Word32 Word32 := 
-  shift z.
+  shift_const z.
 
 Definition rotate32 z {term : Core.Algebra} : term Word32 Word32 := 
-  rotate z.
+  rotate_const z.
 
 Definition hashBlock {term : Core.Algebra} : term (Word256 * Word512) Word256 :=
 let a32 := add32 in
@@ -98,14 +98,14 @@ let odiag := O diag in
 let idiag := I diag in
 let bigDiag := O I I H &&& I O O H in
 let part1Schedule := odiag &&& bigDiag in
-let smallSigma0 := rotate32 7 &&& rotate32 18 &&& shift32 3 >>> x32 in
-let smallSigma1 := rotate32 17 &&& rotate32 19 &&& shift32 10 >>> x32 in
+let smallSigma0 := rotate32 (-7) &&& rotate32 (-18) &&& shift32 (-3) >>> x32 in
+let smallSigma1 := rotate32 (-17) &&& rotate32 (-19) &&& shift32 (-10) >>> x32 in
 let smallSigma := (O O O (O H &&& (I H >>> smallSigma0)) >>> a32)
              &&& (I (O O I H &&& (I I O H >>> smallSigma1)) >>> a32) >>> a32 in
 let schedule := (O part1Schedule &&& (O idiag &&& (O I I I H &&& I (O O O H))))
            &&& (I part1Schedule &&& (I idiag &&& (I I I I H &&& smallSigma))) in
-let bigSigma0 := rotate32 2 &&& rotate32 13 &&& rotate32 22 >>> x32 in
-let bigSigma1 := rotate32 6 &&& rotate32 11 &&& rotate32 25 >>> x32 in
+let bigSigma0 := rotate32 (-2) &&& rotate32 (-13) &&& rotate32 (-22) >>> x32 in
+let bigSigma1 := rotate32 (-6) &&& rotate32 (-11) &&& rotate32 (-25) >>> x32 in
 let t1 := (O H &&& I I O O O O H >>> a32) &&& I O (I (I I H &&& ((O O H >>> bigSigma1) &&& (O O H &&& diag >>> chWord32) >>> a32)) >>> a32) >>> a32 in
 let t12 := O ((O I H &&& I H >>> majWord32) &&& (O (O H &&& (I H >>> bigSigma0)) >>> a32)) >>> a32 in
 let t1d := O O O H &&& I O O H >>> a32 in
@@ -194,15 +194,16 @@ apply (bitwiseTri_correct f);[|intros [[] | []] [[] | []] [[] | []]];
 reflexivity.
 Qed.
 
-Lemma shift32_correct z (Hz : (0 <= z <= Int.max_unsigned)%Z) (x : Word32) :
-  Int.repr (toZ (|[shift32 z]| x)) = general_lemmas.Shr z (Int.repr (toZ x)).
+Lemma shift32_correct z (Hz : (0 <= (-z) <= Int.max_unsigned)%Z) (x : Word32) :
+  Int.repr (toZ (|[shift32 z]| x)) = general_lemmas.Shr (-z) (Int.repr (toZ x)).
 Proof.
 unfold general_lemmas.Shr.
 apply Int.same_bits_eq; intros i Hi.
 rewrite Int.testbit_repr by assumption.
 rewrite Int.bits_shru by assumption.
 unfold shift32.
-rewrite shift_correct by assumption.
+rewrite <-(Z.opp_involutive z) at 1.
+rewrite shift_const_correct by assumption.
 rewrite Int.unsigned_repr by assumption.
 destruct (Coqlib.zlt _ _) as [Hiz|Hiz].
  rewrite Int.testbit_repr by lia.
@@ -215,7 +216,7 @@ lia.
 Qed.
 
 Lemma rotate32_correct z (x : Word32) :
-  Int.repr (toZ (|[rotate32 z]| x)) = SHA256.Rotr z (Int.repr (toZ x)).
+  Int.repr (toZ (|[rotate32 z]| x)) = SHA256.Rotr (-z) (Int.repr (toZ x)).
 Proof.
 unfold SHA256.Rotr.
 apply Int.same_bits_eq; intros i Hi.
@@ -223,8 +224,9 @@ rewrite Int.bits_ror by assumption.
 rewrite Int.testbit_repr by assumption.
 rewrite Int.testbit_repr by (apply Z_mod_lt; constructor).
 unfold rotate32.
-rewrite rotate_correct by assumption.
-rewrite Int.unsigned_repr_eq, <- (Zplus_mod_idemp_r (z mod Int.modulus))%Z, <- Znumtheory.Zmod_div_mod; try constructor.
+rewrite <-(Z.opp_involutive z) at 1.
+rewrite rotate_const_correct_word by assumption.
+rewrite Int.unsigned_repr_eq, <- (Zplus_mod_idemp_r ((-z) mod Int.modulus))%Z, <- Znumtheory.Zmod_div_mod; try constructor.
  rewrite Zplus_mod_idemp_r.
  reflexivity.
 apply Znumtheory.Zmod_divide; auto with zarith.
@@ -260,11 +262,12 @@ replace (|[compression]| (h,b)) with
  simpl fold_right at 1.
  set (fr0 := fold_right comp _ _);fold (Word256) in fr0.
  set (fr1 := fold_right _ _ _).
- unfold comp; simpl.
+ unfold comp; simpl; fold Word32.
  match goal with
-  |- _ = fr1 ?p => generalize p
- end;
- intros p;change (tySem (Word32*(Word256*Word512))) in p;revert p.
+  |- _ = fr1 ?p => set (p0:=p)
+ end.
+ change (step _) with (step p0).
+ generalize p0; clear p0.
  clear h b.
  induction ks;[reflexivity|].
  intros p.
@@ -401,6 +404,7 @@ Lemma xor3Word32_Parametric {term1 term2 : Core.Algebra} (R : Core.Parametric.Re
   R _ _ xor3Word32 xor3Word32.
 Proof.
 unfold xor3Word32.
+repeat apply buildBitwiseTri_Parametric.
 auto with parametricity.
 Qed.
 Hint Immediate xor3Word32_Parametric : parametricity.
@@ -409,6 +413,7 @@ Lemma chWord32_Parametric {term1 term2 : Core.Algebra} (R : Core.Parametric.Rel 
   R _ _ chWord32 chWord32.
 Proof.
 unfold chWord32.
+repeat apply buildBitwiseTri_Parametric.
 auto with parametricity.
 Qed.
 Hint Immediate chWord32_Parametric : parametricity.
@@ -417,6 +422,7 @@ Lemma majWord32_Parametric {term1 term2 : Core.Algebra} (R : Core.Parametric.Rel
   R _ _ majWord32 majWord32.
 Proof.
 unfold majWord32.
+repeat apply buildBitwiseTri_Parametric.
 auto with parametricity.
 Qed.
 Hint Immediate majWord32_Parametric : parametricity.
@@ -457,7 +463,7 @@ Hint Immediate hashBlock_Parametric : parametricity.
 Require Import Simplicity.MerkleRoot.
 
 Fact identityRoot_hashBlock : map Byte.unsigned (hash256_to_bytelist (identityRoot hashBlock)) =
-  map Byte.unsigned (sha.functional_prog.hexstring_to_bytelist "c03041ed97dcadae702ee60060641d7a1040a4ccefb92f0535d02b754649e4f4").
+  map Byte.unsigned (sha.functional_prog.hexstring_to_bytelist "609cc1459375db728f2172c962807e3161df4cced6592d2c4e594a7779ab3175").
 Proof.
 vm_compute.
 reflexivity.
