Coq/Simplicity/Word.v
@@ -3,6 +3,7 @@ Require Import List.
 Require Import ZArith.
 Require Import Simplicity.Util.Arith.
 Require Import Lia.
+Require Coq.Vectors.Vector.
 Require compcert.lib.Integers.
 
 Require Import Simplicity.Ty.
@@ -18,11 +19,22 @@ Local Open Scope ty_scope.
 Local Open Scope term_scope.
 Local Open Scope semantic_scope.
 
-Fixpoint Word (n : nat) :=
+Fixpoint Vector X (n : nat) :=
 match n with
-| 0 => Bit
-| S n => let rec := Word n in Prod rec rec
+| 0 => X
+| S n => let rec := Vector X n in Prod rec rec
 end.
+
+Lemma VectorPromote {X n} : Vector X (S n) = Vector (X * X) n.
+Proof.
+induction n.
+- reflexivity.
+- cbn.
+  rewrite <-!IHn.
+  reflexivity.
+Defined.
+
+Definition Word := Vector Bit.
 
 Module ToZ.
 
@@ -322,129 +334,141 @@ Definition multiplier {n : nat} {term : Core.Algebra} : term (Word n * Word n) (
 
 End Arith.
 
-Section BitVector.
+Section Vector.
+
+Definition build_fill {C X} {term : Core.Algebra} 
+  (rec : term C X) : term C (X * X) := rec &&& rec.
+
+Fixpoint fill {C X n} {term : Core.Algebra} (t : term C X) : term C (Vector X n) :=
+match n with
+| 0 => t
+| (S n) => build_fill (fill t)
+end.
 
 Definition buildBitwiseTri {W} {term : Core.Algebra} (rec : term (W * (W * W)) W) :
   term ((W * W) * ((W * W) * (W * W))) (W * W) :=
     (O O H &&& (I O O H &&& I I O H) >>> rec)
 &&& (O I H &&& (I O I H &&& I I I H) >>> rec).
 
-Fixpoint bitwiseTri {n : nat} {term : Core.Algebra} (op : term (Bit * (Bit * Bit)) Bit) :
-  term (Word n * (Word n * Word n)) (Word n) :=
+Fixpoint bitwiseTri {X} {n : nat} {term : Core.Algebra} (op : term (X * (X * X)) X) :
+  term (Vector X n * (Vector X n * Vector X n)) (Vector X n) :=
 match n with
 | 0 => op
 | S n => buildBitwiseTri (bitwiseTri op)
 end.
 
-Fixpoint subseq0_le {n m} {term : Core.Algebra} : term (Word n) (Word (m + n)) :=
-match m with
-| 0 => iden
-| S m => (unit >>> zero) &&& subseq0_le
-end.
+Definition build_leftmost {V X} {term : Core.Algebra} 
+  (rec : term V X) : term (V * V) X := take rec.
 
-Fixpoint subseq0_ge {n m} {term : Core.Algebra} : term (Word (m + n)) (Word n) :=
-match m with
-| 0 => iden
-| S m => drop subseq0_ge
-end.
-
-Definition subseq0 {n m} {term : Core.Algebra} : term (Word n) (Word m) :=
-match natDiff n m with
-| inl (exist _ i Hi) => eq_rect _ (fun x => term (Word n) (Word x)) subseq0_le _ Hi
-| inr (exist _ i Hi) => eq_rect _ (fun x => term (Word x) (Word m)) subseq0_ge _ Hi
-end.
-
-Fixpoint subseqBit {n} (z:Z) {term : Core.Algebra} : term Bit (Word n) :=
+Fixpoint leftmost {X n} {term : Core.Algebra} : term (Vector X n) X :=
 match n with
-| 0 => match (Z.eq_dec z 0)%Z with
-       | Specif.left _ => iden
-       | Specif.right _ => false
-       end
-| S n => subseqBit (z + two_power_nat n) &&& subseqBit z
+| 0 => iden
+| S n => build_leftmost leftmost
 end.
 
-Fixpoint subseqPair {n m} (z:Z) {term : Core.Algebra} (rec : forall {m}, Z -> term (Word n) (Word m)) : term (Word (S n)) (Word m) :=
-match (Z.eq_dec z 0)%Z with
-| Specif.left _ => subseq0
-| Specif.right _ =>
-  match Z_lt_le_dec z (two_power_nat n) with
-  | Specif.right _ =>
-    match Z_lt_le_dec z (two_power_nat (S n)) with
-    | Specif.right _ => unit >>> zero
-    | Specif.left _ => take (rec (z - two_power_nat n)%Z)
-    end
-  | Specif.left Hz0 =>
-    match Z_lt_le_dec (two_power_nat n) (z + two_power_nat m) with
-    | Specif.right _ => 
-      match Z_lt_le_dec 0 (z + two_power_nat m) with
-      | Specif.right _ => unit >>> zero
-      | Specif.left _ => drop (rec z)
-      end
-    | Specif.left Hz1 =>
-      match m return ((two_power_nat n < z + two_power_nat m)%Z -> term (Word (S n)) (Word m)) with
-      | 0 => fun Hz1 => False_rect _ (Zlt_not_le _ _ Hz0 (Zlt_succ_le _ _ Hz1))
-      | S m => fun _ => subseqPair (z + two_power_nat m) (@rec) &&& subseqPair z (@rec)
-      end Hz1
-    end
+Definition build_rightmost {V X} {term : Core.Algebra} 
+  (rec : term V X) : term (V * V) X := drop rec.
+
+Fixpoint rightmost {X n} {term : Core.Algebra} : term (Vector X n) X :=
+match n with
+| 0 => iden
+| S n => build_rightmost rightmost
+end.
+
+Definition build_full_left_shift1 {X W} {term : Core.Algebra} 
+  (rec : term (W * X) (X * W)) : term ((W * W) * X) (X * (W * W)) :=
+   O O H &&& (O I H &&& I H >>> rec) >>> (O H &&& I O H >>> rec) &&& I I H >>> O O H &&& (O I H &&& I H).
+
+Fixpoint full_left_shift1 {X n} {term : Core.Algebra} :
+  term (Vector X n * X) (X * Vector X n) :=
+match n with
+| 0 => iden
+| S n => build_full_left_shift1 full_left_shift1
+end.
+
+Definition build_full_right_shift1 {X W} {term : Core.Algebra} 
+  (rec : term (X * W) (W * X)) : term (X * (W * W)) ((W * W) * X) :=
+(O H &&& I O H >>> rec) &&& I I H >>> O O H &&& (O I H &&& I H >>> rec) >>> (O H &&& I O H) &&& I I H.
+
+Fixpoint full_right_shift1 {X n} {term : Core.Algebra} :
+  term (X * Vector X n) (Vector X n * X) :=
+match n with
+| 0 => iden
+| S n => build_full_right_shift1 full_right_shift1
+end.
+
+Definition left_shift1 {X n} {term : Core.Algebra} (t : term Unit X) : term (Vector X n) (Vector X n) :=
+iden &&& (unit >>> t) >>> full_left_shift1 >>> I H.
+
+Fixpoint left_shift_const_by {X n} {term : Core.Algebra} (t : term Unit X) (p : positive) 
+ : term (Vector X n) (Vector X n) :=
+if (Zpower_nat 2 n <=? Zpos p)%Z then
+ unit >>> fill t else
+match n with 
+| 0 => iden
+| (S n0) => match p with
+  | xH => left_shift1 t
+  | xO p0 => eq_rect _ (fun x => term x x) (left_shift_const_by (t &&& t) p0) _ (eq_sym VectorPromote)
+  | xI p0 => left_shift1 t >>> eq_rect _ (fun x => term x x) (left_shift_const_by (t &&& t) p0) _ (eq_sym VectorPromote)
   end
 end.
 
-Fixpoint subseq {n m} (z:Z) {term : Core.Algebra} : term (Word n) (Word m) :=
-match n with
-| 0 => subseqBit z
-| S n => subseqPair z (fun m z => @subseq n m z term)
-end.
+Definition right_shift1 {X n} {term : Core.Algebra} (t : term Unit X) : term (Vector X n) (Vector X n) :=
+(unit >>> t) &&& iden >>> full_right_shift1 >>> O H.
 
-Definition shift {n} (z:Z) {term : Core.Algebra} : term (Word n) (Word n) := subseq z.
-
-Fixpoint subseqWrap0_le {n m} {term : Core.Algebra} : term (Word n) (Word (m + n)) :=
-match m with
+Fixpoint right_shift_const_by {X n} {term : Core.Algebra} (t : term Unit X) (p : positive) 
+ : term (Vector X n) (Vector X n) :=
+if (Zpower_nat 2 n <=? Zpos p)%Z then
+ unit >>> fill t else
+match n with 
 | 0 => iden
-| S m => let rec := subseqWrap0_le in rec &&& rec
-end.
-
-Definition subseqWrap0 {n m} {term : Core.Algebra} : term (Word n) (Word m) :=
-match natDiff n m with
-| inl (exist _ i Hi) => eq_rect _ (fun x => term (Word n) (Word x)) subseqWrap0_le _ Hi
-| inr (exist _ i Hi) => eq_rect _ (fun x => term (Word x) (Word m)) subseq0_ge _ Hi
-end.
-
-Fixpoint subseqWrapPair {n m} (z:Z) {term : Core.Algebra} (rec : forall {m}, Z -> term (Word n) (Word m)) : term (Word (S n)) (Word m) :=
-let z := (z mod (two_power_nat (S n)))%Z in (* shadow old value of z to take it out of scope *)
-match (Z.eq_dec z 0)%Z with
-| Specif.left _ => subseqWrap0
-| Specif.right _ =>
-  match (Z_lt_le_dec z (two_power_nat n)) with
-  | Specif.left _ =>
-    match m with
-    | 0 => drop (rec z)
-    | S m =>
-      match Z_lt_le_dec (two_power_nat n) (z + two_power_nat (S m)) with
-      | Specif.right _ => drop (rec z)
-      | Specif.left _ => subseqWrapPair (z + two_power_nat m) (@rec) &&&  subseqWrapPair z (@rec)
-      end
-    end
-  | Specif.right _ => 
-    match m with
-    | 0 => take (rec (z - two_power_nat n)%Z)
-    | S m =>
-      match Z_lt_le_dec (two_power_nat (S n)) (z + two_power_nat (S m)) with
-      | Specif.left _ => subseqWrapPair (z + two_power_nat m) (@rec) &&& subseqWrapPair z (@rec)
-      | Specif.right _ => take (rec (z - two_power_nat n)%Z)
-      end
-    end
+| (S n0) => match p with
+  | xH => right_shift1 t
+  | xO p0 => eq_rect _ (fun x => term x x) (right_shift_const_by (t &&& t) p0) _ (eq_sym VectorPromote)
+  | xI p0 => right_shift1 t >>> eq_rect _ (fun x => term x x) (right_shift_const_by (t &&& t) p0) _ (eq_sym VectorPromote)
   end
 end.
 
-Fixpoint subseqWrap {n m} (z:Z) {term : Core.Algebra} : term (Word n) (Word m) :=
-match n with
-| 0 => subseqWrap0
-| S n => subseqWrapPair z (fun m z => @subseqWrap n m z term)
+Definition shift_const_by {X n} {term : Core.Algebra} (t : term Unit X) (c : Z) 
+ : term (Vector X n) (Vector X n) :=
+match c with
+| Z0 => iden
+| Zpos p => left_shift_const_by t p
+| Zneg p => right_shift_const_by t p
 end.
 
-Definition rotate {n} (z:Z) {term : Core.Algebra} : term (Word n) (Word n) := subseqWrap z.
+Definition shift_const {n} {term : Core.Algebra} : Z -> term (Vector Bit n) (Vector Bit n) :=
+  shift_const_by false.
 
-End BitVector.
+Definition left_rotate1 {X n} {term : Core.Algebra} : term (Vector X n) (Vector X n) :=
+iden &&& leftmost >>> full_left_shift1 >>> I H.
+
+Definition right_rotate1 {X n} {term : Core.Algebra} : term (Vector X n) (Vector X n) :=
+rightmost &&& iden >>> full_right_shift1 >>> O H.
+
+Fixpoint rotate_const_list {X n} {term : Core.Algebra} (z : Z) 
+ : list (term (Vector X n) (Vector X n)) :=
+match n with 
+| 0 => []
+| (S n0) =>
+  if Z.even z
+  then eq_rect _ (fun x => list (term x x)) (rotate_const_list (Z.div z 2)%Z) _ (eq_sym VectorPromote)
+  else if Z.even (Z.div z 2)
+  then left_rotate1 :: eq_rect _ (fun x => list (term x x)) (rotate_const_list (Z.div z 2)%Z) _ (eq_sym VectorPromote)
+  else right_rotate1 :: eq_rect _ (fun x => list (term x x)) (rotate_const_list (Z.div (z + 1) 2)%Z) _ (eq_sym VectorPromote)
+end.
+
+Fixpoint foldr_comp {X} {term : Core.Algebra} (l : list (term X X)) : term X X :=
+match l with
+| [] => iden
+| i::[] => i
+| i::l => i >>> foldr_comp l
+end.
+
+Definition rotate_const {X n} {term : Core.Algebra} (z : Z) : term (Vector X n) (Vector X n) :=
+foldr_comp (rotate_const_list z).
+
+End Vector.
 
 End Definitions.
 
@@ -460,6 +484,7 @@ Lemma fullAdder_correct n : forall (a b : Word n) (c : Bit),
 Proof.
 induction n. { intros [[] | []] [[] | []] [[] | []]; reflexivity. }
 intros [ahi alo] [bhi blo] c.
+fold Word in *.
 cbn -[toZ]; fold tySem; fold (tySem Bit).
 rewrite (toZ_Pair ahi alo), (toZ_Pair bhi blo).
 set (C := two_power_nat _).
@@ -498,6 +523,7 @@ Proof.
 induction n. { intros [[] | []] [[] | []] [[] | []] [[] | []]; reflexivity. }
 intros [ahi alo] [bhi blo] [chi clo] [dhi dlo].
 cbn -[toZ]; fold tySem; fold (tySem Bit).
+fold Word in *.
 rewrite (toZ_Pair ahi alo), (toZ_Pair bhi blo), (toZ_Pair chi clo), (toZ_Pair dhi dlo).
 set (C := two_power_nat _).
 transitivity ((toZ ahi * C + toZ alo) * toZ bhi * C +
@@ -507,6 +533,7 @@ rewrite <- 2!IHn.
 destruct (|[fullMultiplier]| ((alo, blo), (clo, dlo))) as [c0 rOO]; clear clo dlo.
 destruct (|[fullMultiplier]| ((ahi, blo), (chi, dhi))) as [c1 c2]; clear chi dhi blo.
 cbn [fst snd].
+fold Word in *.
 rewrite (toZ_Pair c1 c2), (toZ_Pair c0 rOO); fold C.
 transitivity ((toZ ahi * toZ bhi + toZ c1) * C * C +
  (toZ bhi * toZ alo + toZ c2 + toZ c0) * C + toZ rOO)%Z;
@@ -514,6 +541,7 @@ transitivity ((toZ ahi * toZ bhi + toZ c1) * C * C +
 rewrite <- IHn.
 destruct (|[fullMultiplier]| ((bhi, alo), (c2, c0))) as [c3 rOI]; clear c2 c0 alo.
 cbn [fst snd].
+fold Word in *.
 rewrite (toZ_Pair c3 rOI); fold C.
 transitivity ((toZ ahi * toZ bhi + toZ c3 + toZ c1) * C * C + toZ rOI * C + toZ rOO)%Z;
  [|ring].
@@ -534,13 +562,71 @@ rewrite fullMultiplier_correct, zero_correct.
 ring.
 Qed.
 
+Import Coq.Vectors.Vector.VectorNotations.
+
+Fixpoint replicate {X} (x : X) n : Vector.t X n :=
+match n return Vector.t X n with 
+| 0 => []
+| S m => (x :: replicate x m)
+end.
+
+Lemma replicate_append {X} (x : X) n m : replicate x n ++ replicate x m = replicate x (n + m).
+Proof.
+induction n.
+- reflexivity.
+- cbn.
+  f_equal.
+  assumption.
+Qed.
+
+Lemma nth_replicate {X n i} (x : X) (ix : i < n) : Vector.nth_order (replicate x n) ix = x.
+Proof.
+revert i ix.
+induction n;[|intros [|i] Hi].
+- lia.
+- simpl.
+  rewrite Vector.nth_order_hd.
+  reflexivity.
+- assert (Hin : i < n) by lia.
+  rewrite <- (Vector.nth_order_tl _ _ _ _ Hin).
+  apply IHn.
+Qed.
+
+Lemma mul_2_r n : (2 * n = n + n)%nat.
+Proof.
+cbn.
+f_equal.
+induction n.
+- reflexivity.
+- cbn.
+  f_equal.
+  assumption.
+Defined.
+
+Fixpoint flatten {X n} : Vector X n -> Vector.t X (2^n) :=
+match n return Vector X n -> Vector.t X (2^n) with
+| 0 => fun v => [v]
+| S n => fun v => eq_rect _ (Vector.t X) (flatten (fst v) ++ flatten (snd v)) _ (eq_sym (mul_2_r (2^n)))
+end.
+
+Lemma fill_correct {C X n} (t : Arrow C X) (c : C) : flatten (|[ fill t ]| c) = replicate (|[ t ]| c) (2^n).
+Proof.
+induction n.
+- reflexivity.
+- cbn.
+  rewrite IHn.
+  generalize ( (mul_2_r (2 ^ n))).
+  cbn; intros ->; cbn.
+  apply replicate_append.
+Qed.
+
 Definition TrinarySpec {n} (f : bool -> bool -> bool -> bool) (term : Arrow (Word n * (Word n * Word n)) (Word n)) :=
   forall (x y z : Word n) i, (Z.testbit (toZ (term (x,(y,z)))) i = f (Z.testbit (toZ x) i) (Z.testbit (toZ y) i) (Z.testbit (toZ z) i))%Z.
 
 Lemma bitwiseTri_correct {n} (f : bool -> bool -> bool -> bool) (op : Arrow (Bit * (Bit * Bit)) Bit)
     (Hf : f Datatypes.false Datatypes.false Datatypes.false = Datatypes.false)
     (Hop : (forall (a b c : Bit), toBool (op (a,(b,c))) = f (toBool a) (toBool b) (toBool c))) :
-  forall (a b c : Word n) i, (Z.testbit (toZ (bitwiseTri op (a,(b,c)))) i = f (Z.testbit (toZ a) i) (Z.testbit (toZ b) i) (Z.testbit (toZ c) i))%Z.
+  TrinarySpec (n:=n) f (bitwiseTri op).
 Proof.
 induction n.
  intros a b c i.
@@ -561,211 +647,1301 @@ destruct (Z_lt_le_dec i (two_power_nat n)) as [Hi|Hi]; cbn;
 ]; auto.
 Qed.
 
-Let subseqSpec n m z (t : Arrow (Word n) (Word m)) :=
-  forall x i, (0 <= i < two_power_nat m)%Z -> Z.testbit (toZ (t x)) i = Z.testbit (toZ x) (i + z)%Z.
+Definition pow_succ n : (2^n = S (pred (2^n)))%nat.
+case_eq (2^n).
+- abstract (intros H;elim (Nat.pow_nonzero 2 n);lia).
+- reflexivity.
+Defined.
 
-Lemma subseq0_ge_correct n m : subseqSpec (m + n) n 0 subseq0_ge.
+Definition pow_hd {X n} (v : Vector.t X (2^n)) : X :=
+Vector.hd (eq_rect _ (Vector.t X) v _ (pow_succ n)).
+
+Definition pow_last {X n} (v : Vector.t X (2^n)) : X :=
+Vector.last (eq_rect _ (Vector.t X) v _ (pow_succ n)).
+
+Lemma hd_flatten {X n} (v0 v1 : Vector X n):
+  pow_hd (@flatten X (S n) (v0,v1)) = pow_hd (@flatten X n v0).
 Proof.
-intros x i Hi; clear - Hi.
-rewrite Z.add_0_r.
-induction m.
- reflexivity.
-destruct x as [xhi xlo]; simpl.
-rewrite testbitToZLo.
- apply IHm; assumption.
-eapply Z.lt_le_trans;[apply Hi|].
-auto using two_power_nat_le with arith.
-Qed.
-
-Lemma subseq0_le_correct n m : subseqSpec n (m + n) 0 subseq0_le.
-Proof.
-intros x i Hi; clear - Hi.
-rewrite Z.add_0_r.
-induction m.
- reflexivity.
-simpl.
-destruct (Z_lt_le_dec i (two_power_nat (m + n))) as [Hi0|Hi0].
-- rewrite testbitToZLo by auto.
-  apply IHm; tauto.
-- rewrite testbitToZHi by auto.
-  rewrite zero_correct, Z.bits_0, toZ_mod, two_power_nat_equiv.
-  rewrite Z.mod_pow2_bits_high;[reflexivity|].
-  split;[auto with zarith|].
-  rewrite bitSize_Word.
-  etransitivity;[|apply Hi0].
-  auto using two_power_nat_le with arith.
-Qed.
-
-Lemma subseq0_correct n m : subseqSpec n m 0 subseq0.
-Proof.
-unfold subseq0.
-destruct natDiff as [[i <-] | [i <-]]; cbn;
-[apply subseq0_le_correct
-|apply subseq0_ge_correct].
-Qed.
-
-Lemma subseqBit_correct n z : subseqSpec 0 n z (subseqBit z).
-Proof.
-intros x; clear.
-revert z; induction n; intros z i Hi; simpl.
- change (two_power_nat 0) with 1%Z in Hi.
- replace i with 0%Z by auto with zarith; clear Hi.
- destruct Z.eq_dec as [->|Hz];[reflexivity|].
- destruct x as [[] | []];cbn;[rewrite Z.bits_0; reflexivity|].
- destruct (not_Zeq _ _ Hz) as [Hz0|Hz0];
- [rewrite Z.testbit_neg_r
- |rewrite Z.bits_above_log2];
- auto with zarith.
-destruct (Z_lt_le_dec i (two_power_nat n)) as [Hi0|Hi0].
-- rewrite testbitToZLo by auto.
-  apply IHn; auto with zarith.
-- rewrite two_power_nat_S in Hi.
-  rewrite testbitToZHi, IHn by auto with zarith.
-  f_equal; ring.
-Qed.
-
-Lemma subseqPair_correct n m z rec (Hrec : forall m z, subseqSpec n m z (rec m z)) :
-  subseqSpec (S n) m z (subseqPair z rec).
-Proof.
-unfold subseqSpec in *.
-revert z; induction m; intros z [xhi xlo] i Hi; cbn -[toZ zero subseq0 Word];
-(destruct Z.eq_dec as [->|];[apply subseq0_correct; auto|]);
- repeat destruct Z_lt_le_dec; try rewrite zero_correct;
- try solve
- [destruct Zlt_not_le
- |rewrite testbitToZLo;[apply Hrec|]; auto with zarith
- |rewrite Z.bits_0, Z.testbit_neg_r; auto with zarith
- |rewrite testbitToZHi, <- Z.add_sub_assoc;[apply Hrec|]; auto with zarith
- |rewrite Z.bits_0, toZ_mod, two_power_nat_equiv, bitSize_Word, Z.mod_pow2_bits_high;
-   rewrite <- bitSize_Word in *;
-   auto with zarith].
-destruct (Z_lt_le_dec i (two_power_nat m)) as [Hi0|Hi0].
-- rewrite (testbitToZLo _ _ Hi0), IHm; auto with zarith.
-- rewrite two_power_nat_S in Hi.
-  rewrite (testbitToZHi _ _ Hi0), IHm by auto with zarith.
-  f_equal; ring.
-Qed.
-
-Lemma subseq_correct n : forall m z, subseqSpec n m z (subseq z).
-Proof.
-induction n; intros; cbn;
-auto using subseqBit_correct, subseqPair_correct.
-Qed.
-
-Lemma shift_correct n z (x : Word n) i (Hi : (0 <= i < two_power_nat n)%Z) :
-  Z.testbit (toZ (|[shift z]| x)) i = Z.testbit (toZ x) (i + z)%Z.
-Proof.
-exact (subseq_correct n z x Hi).
-Qed.
-
-Let subseqWrapSpec n m z (t : Arrow (Word n) (Word m)) :=
-  forall x i, (0 <= i < two_power_nat m)%Z ->
-  Z.testbit (toZ (t x)) i = Z.testbit (toZ x) (Zmod (i + z) (two_power_nat  n)).
-
-Lemma subseqWrap0_ge_correct n m : subseqWrapSpec (m + n) n 0 subseq0_ge.
-Proof.
-intros x i Hi.
-rewrite Z.mod_small;[apply subseq0_ge_correct|split]; auto with zarith.
-apply Z.lt_le_trans with (two_power_nat n);
-auto using two_power_nat_le with zarith.
-Qed.
-
-Lemma subseqWrap0_le_correct n m : subseqWrapSpec n (m + n) 0 subseqWrap0_le.
-Proof.
-intros x i Hi; clear - Hi.
-rewrite Z.add_0_r.
-revert i Hi; induction m; intros i Hi.
- rewrite Z.mod_small; auto.
-simpl.
-destruct (Z_lt_le_dec i (two_power_nat (m + n))) as [Hi0|Hi0]; simpl in *.
- rewrite testbitToZLo by auto.
- apply IHm; tauto.
-rewrite two_power_nat_S in Hi.
-rewrite testbitToZHi, IHm by auto with zarith.
-rewrite two_power_nat_plus.
-replace (i - two_power_nat m * two_power_nat n)%Z with (i + (- two_power_nat m) * two_power_nat n)%Z by ring.
-rewrite Z_mod_plus_full.
+unfold pow_hd; cbn.
+generalize (mul_2_r (2 ^ n)) (pow_succ n) (pow_succ (S n)).
+  change (2 * 2 ^ n)%nat with (2 ^ (S n))%nat.
+change (2 ^ n + (2 ^ n + 0))%nat with (2 ^ (S n))%nat.
+intros -> e0 e1; simpl.
+cut (forall a b (e0 : a = S (Init.Nat.pred a))
+(e1 : (a + b)%nat = S (Init.Nat.pred (a + b)))
+  (v : Vector.t X a) (w : Vector.t X b),
+Vector.hd
+  (eq_rect (a + b)%nat (Vector.t X) (v ++ w)
+     (S (Init.Nat.pred (a + b))) e1) =
+Vector.hd
+  (eq_rect a (Vector.t X) v (S (Init.Nat.pred a)) e0));
+[intros H0; apply H0|clear e0 e1].
+intros a b -> e; simpl.
+elim e using K_dec_set;[apply Nat.eq_dec|simpl].
+intros v.
+rewrite (Vector.eta v).
 reflexivity.
 Qed.
 
-Lemma subseqWrap0_correct n m : subseqWrapSpec n m 0 subseqWrap0.
+Lemma leftmost_correct {X n v} : |[ leftmost ]| v = pow_hd (@flatten X n v).
 Proof.
-unfold subseqWrap0.
-destruct natDiff as [[i <-] | [i <-]]; cbn;
-[apply subseqWrap0_le_correct
-|apply subseqWrap0_ge_correct].
+induction n.
+- reflexivity.
+- cbn.
+  rewrite IHn; clear IHn.
+  symmetry.
+  apply hd_flatten.
 Qed.
 
-Lemma subseqWrapBit_correct n z : subseqWrapSpec 0 n z subseqWrap0.
+Lemma Vector_eta_shift {X n} (v : Vector.t X (S n)) : v = Vector.shiftin (Vector.last v) (Vector.shiftout v).
 Proof.
-intros x i; rewrite Z.mod_1_r; revert x i.
-unfold subseqWrap0.
-destruct natDiff as [[i0 <-] | [i0 Hi0]]; cbn -[Word Z.testbit toZ].
- intros x i Hi; rewrite plus_0_r in Hi.
- revert i Hi; induction i0; intros i Hi.
-  change (two_power_nat 0) with 1%Z in Hi.
-  replace i with 0%Z by auto with zarith.
+elim v using Vector.rectS.
+- reflexivity.
+- simpl. intros a c w IH. f_equal. assumption.
+Qed.
+
+Lemma rightmost_correct {X n v} : |[ rightmost ]| v = pow_last (@flatten X n v).
+Proof.
+induction n.
+- reflexivity.
+- cbn.
+  rewrite IHn; clear IHn.
+  unfold pow_last.
+  generalize (mul_2_r (2 ^ n)) (pow_succ n) (pow_succ (S n)).
+    change (2 * 2 ^ n)%nat with (2 ^ (S n))%nat.
+  change (2 ^ n + (2 ^ n + 0))%nat with (2 ^ (S n))%nat.
+  intros -> e0 e1; simpl.
+  cut (forall a b (e0 : b = S (Init.Nat.pred b))
+  (e1 : (a + b)%nat = S (Init.Nat.pred (a + b)))
+  (v : Vector.t X a) (w : Vector.t X b),
+Vector.last
+  (eq_rect b (Vector.t X) w (S (Init.Nat.pred b)) e0) =
+Vector.last
+  (eq_rect (a + b)%nat (Vector.t X) (v ++ w)
+     (S (Init.Nat.pred (a + b))) e1));
+  [intros H0; apply H0|clear v e0 e1].
+  intros a b ->; simpl.
+  replace (Init.Nat.pred (a + S (Init.Nat.pred b))) with 
+    (a + Init.Nat.pred b)%nat by (rewrite Nat.add_succ_r; reflexivity).
+  intros e v w.
+  transitivity (Vector.last (Vector.shiftin (Vector.last w) (v ++ Vector.shiftout w)));
+  [rewrite Vector.shiftin_last; reflexivity|].
+  f_equal.
+  revert e w.
+  generalize (pred b); clear b.
+  (* This shiftin/app/shiftout lemma could perhaps be generalized *)
+  induction v.
+  + simpl.
+    intros b e w.
+    elim e using K_dec_set;[apply Nat.eq_dec|clear e].
+    simpl.
+    symmetry.
+    apply Vector_eta_shift.
+  + simpl.
+    intros b e w.
+    assert (e0 : (n0 + S b)%nat = S (n0 + b)) by lia.
+    rewrite (IHv b e0).
+    generalize (v ++ w).
+    revert e.
+    rewrite e0.
+    intros e.
+    elim e using K_dec_set;[apply Nat.eq_dec|reflexivity].
+Qed.
+
+Definition map_fst {A B C} (f : A -> B) (v : A * C) : B * C := (f (fst v), snd v).
+Definition map_snd {A B C} (f : B -> C) (v : A * B) : A * C := (fst v, f (snd v)).
+
+Lemma tail_shiftin {X n} x (v: Vector.t X (S n)) :
+  Vector.tl (Vector.shiftin x v) = Vector.shiftin x (Vector.tl v).
+Proof.
+rewrite (Vector.eta v).
+reflexivity.
+Qed.
+
+Lemma shiftin_append {X n m} (e : (n + S m = S (n + m))%nat) x (v0 : Vector.t X n) (v1 : Vector.t X m) :
+  Vector.shiftin x (v0 ++ v1) = eq_rect _ (Vector.t X) (v0 ++ (Vector.shiftin x v1)) _ e.
+Proof.
+revert e.
+induction v0.
+- cbn; intros e.
+  elim e using K_dec_set;[apply Nat.eq_dec|reflexivity].
+- intros e.
+  assert (e0 : (n + S m)%nat = S (n + m)) by lia.
+  cbn in *.
+  rewrite (IHv0 e0).
+  revert e.
+  rewrite <- e0.
+  cbn.
+  intros e.
+  elim e using K_dec_set;[apply Nat.eq_dec|reflexivity].
+Qed.
+
+Lemma append_shiftin {X n m} (e : (n + S m = S (n + m))%nat) x (v0 : Vector.t X n) (v1 : Vector.t X m) :
+  Vector.shiftin x v0 ++ v1 = eq_rect _ (Vector.t X) (v0 ++ x ::v1) _ e.
+Proof.
+revert e.
+induction v0.
+- cbn; intros e.
+  elim e using K_dec_set;[apply Nat.eq_dec|reflexivity].
+- intros e.
+  assert (e0 : (n + S m)%nat = S (n + m)) by lia.
+  cbn in *.
+  rewrite (IHv0 e0).
+  revert e.
+  rewrite <- e0.
+  cbn.
+  intros e; elim e using K_dec_set;[apply Nat.eq_dec|reflexivity].
+Qed.
+
+Lemma last_flatten {X n} v0 v1 :
+  pow_last (@flatten X (S n) (v0,v1)) = pow_last (@flatten X n v1).
+Proof.
+fold tySem Vector in *.
+unfold pow_last; cbn.
+generalize (mul_2_r (2 ^ n)) (pow_succ n) (pow_succ (S n)).
+  change (2 * 2 ^ n)%nat with (2 ^ (S n))%nat.
+change (2 ^ n + (2 ^ n + 0))%nat with (2 ^ (S n))%nat.
+intros -> e0 e1; simpl.
+cut (forall a b (e0 : b = S (Init.Nat.pred b))
+(e1 : (a + b)%nat = S (Init.Nat.pred (a + b)))
+  (v : Vector.t X a) (w : Vector.t X b),
+Vector.last
+  (eq_rect (a + b)%nat (Vector.t X) (v ++ w)
+     (S (Init.Nat.pred (a + b))) e1) =
+Vector.last
+  (eq_rect b (Vector.t X) w (S (Init.Nat.pred b)) e0));
+[intros H0; apply H0|clear e0 e1].
+intros a b -> e v w; simpl.
+revert e.
+replace (Init.Nat.pred (a + S (Init.Nat.pred b))) with (a + (Init.Nat.pred b))%nat by lia.
+rewrite (Vector_eta_shift w).
+intros e.
+rewrite <- (shiftin_append e).
+rewrite !VectorSpec.shiftin_last.
+reflexivity.
+Qed.
+
+Lemma full_left_shift1_correct {X n v x} :
+  map_snd flatten (|[ full_left_shift1 ]| (v, x)) = (pow_hd (@flatten X n v), Vector.tl (Vector.shiftin x (flatten v))).
+Proof.
+fold tySem in *.
+revert x.
+induction n.
+- reflexivity.
+- destruct v as [v0 v1].
+  simpl.
+  unfold build_full_left_shift1.
+  intros x.
+  unfold map_snd.
+  cbn.
+  injection (IHn v1 x); intros -> ->.
+  set (y := pow_hd (flatten v1)).
+  injection (IHn v0 y); intros -> ->.
+  clear IHn.
+  f_equal.
+  + symmetry. apply hd_flatten.
+  + generalize (mul_2_r (2 ^ n)).
+    cbn; intros ->; cbn.
+    unfold y.
+    generalize (flatten v0) (flatten v1).
+    clear y v0 v1.
+    unfold pow_hd.
+    generalize (pow_succ n).
+    set (Z := pred (2^n)).
+    rewrite (pow_succ n).
+    intros ->.
+    unfold Z; clear Z.
+    cbn.
+    intros v0 v1.
+    rewrite tail_shiftin.
+    rewrite (append_shiftin  (Nat.add_succ_r _ _)).
+    replace (Vector.hd v1) with (Vector.hd (Vector.shiftin x v1)) by
+      (rewrite (Vector.eta v1); reflexivity).
+    rewrite <-Vector.eta.
+    rewrite (shiftin_append (Nat.add_succ_r _ _) x v0 v1).
+    set (e0 := (Nat.add_succ_r _ _)).
+    set (e1 := (Nat.add_succ_r _ _)).
+    clearbody e0 e1.
+    cbn in *.
+    revert e1.
+    rewrite <- e0.
+    intros e; elim e using K_dec_set;[apply Nat.eq_dec|].
+    cbn.
+    rewrite (Vector.eta v0).
+    reflexivity.
+Qed.
+
+Lemma left_shift1_correct {X n v t} :
+  @flatten X n (|[ left_shift1 t ]| v) = Vector.tl (Vector.shiftin (|[ t ]| tt) (flatten v)).
+Proof.
+unfold left_shift1.
+cbn.
+change (flatten (snd _)) with (snd (map_snd flatten (|[full_left_shift1]| (v, t tt)))).
+rewrite full_left_shift1_correct.
+reflexivity.
+Qed.
+
+Lemma shiftout_append {X n m} (e : (n + S m = S (n + m))%nat) (v0 : Vector.t X n) (v1 : Vector.t X (S m)) :
+  Vector.shiftout (eq_rect _ (Vector.t X) (v0 ++ v1) _ e) = v0 ++ (Vector.shiftout v1).
+Proof.
+revert e.
+induction v0.
+- cbn; intros e.
+  elim e using K_dec_set;[apply Nat.eq_dec|reflexivity].
+- intros e.
+  assert (e0 : (n + S m)%nat = S (n + m)) by lia.
+  cbn in *.
+  rewrite <-(IHv0 e0).
+  generalize (v0 ++ v1).
+  revert e.
+  rewrite e0.
+  cbn.
+  intros e.
+  elim e using K_dec_set;[apply Nat.eq_dec|reflexivity].
+Qed.
+
+Lemma full_right_shift1_correct {X n v x} :
+  map_fst flatten (|[ full_right_shift1 ]| (x, v)) = (Vector.shiftout (x :: flatten v), pow_last (@flatten X n v)).
+Proof.
+fold tySem in *.
+revert x.
+induction n.
+- reflexivity.
+- destruct v as [v0 v1].
+  simpl (map_fst _ _).
+  unfold build_full_right_shift1.
+  intros x.
+  unfold map_fst.
+  etransitivity;[cbn|reflexivity].
+  unfold map_fst in IHn.
+  replace (flatten (fst (|[full_right_shift1]| (x, v0)))) with (Vector.shiftout (x :: flatten v0))
+  by (injection (IHn v0 x); auto).
+  replace (snd (|[full_right_shift1]| (x, v0))) with (pow_last (flatten v0))
+  by (injection (IHn v0 x); auto).
+  set (y := pow_last (flatten v0)).
+  replace (flatten (fst (|[full_right_shift1]| (y, v1)))) with (Vector.shiftout (y :: flatten v1))
+  by (injection (IHn v1 y); auto).
+  replace (snd (|[full_right_shift1]| (y, v1))) with (pow_last (flatten v1))
+  by (injection (IHn v1 y); auto).
+  clear IHn.
+  f_equal.
+  + simpl (@flatten X (S n) (v0, v1)).
+    generalize (mul_2_r (2 ^ n)).
+    simpl (2 * _)%nat; simpl (2 ^ (S n))%nat.
+    intros ->.
+    change (Vector.shiftout (x :: flatten v0) ++ Vector.shiftout (y :: flatten v1)
+         = Vector.shiftout (x :: (flatten v0 ++ flatten v1))).
+    unfold y.
+    generalize (flatten v0) (flatten v1).
+    clear y v0 v1.
+    unfold pow_last.
+    generalize (pow_succ n).
+    set (Z := pred (2^n)).
+    rewrite (pow_succ n).
+    intros ->.
+    unfold Z; clear Z.
+    cbn.
+    intros v0 v1.
+    f_equal.
+    change (eq_rect _ (Vector.t X) (Vector.shiftout v0 ++ Vector.last v0 :: Vector.shiftout v1) _ eq_refl
+      = Vector.shiftout (v0 ++ v1)).
+    rewrite <- (eq_trans_sym_inv_r (Nat.add_succ_r _ _)), eq_trans_rew_distr.
+    rewrite <- append_shiftin.
+    rewrite <- Vector_eta_shift.
+    rewrite <- (shiftout_append (Nat.add_succ_r _ _)).
+    generalize (v0 ++ v1).
+    generalize (Nat.add_succ_r (S (Init.Nat.pred (2 ^ n)))
+           (Init.Nat.pred (2 ^ n))).
+    generalize (Nat.add_succ_r (Init.Nat.pred (2 ^ n))
+           (Init.Nat.pred (2 ^ n))).
+    cbn; intros <-; cbn.
+    intros e;elim e using K_dec_set;[apply Nat.eq_dec|].
+    reflexivity.
+  + symmetry. apply last_flatten.
+Qed.
+
+Lemma right_shift1_correct {X n v t} :
+  @flatten X n (|[ right_shift1 t ]| v) = Vector.shiftout (|[ t ]| tt :: flatten v).
+Proof.
+unfold right_shift1.
+etransitivity;[cbn|reflexivity].
+change (flatten (fst _)) with (fst (map_fst flatten (|[full_right_shift1]| (t tt, v)))).
+rewrite full_right_shift1_correct.
+reflexivity.
+Qed.
+
+Lemma nth_order_shiftout {X n i} (v : Vector.t X (S n)) (ix1 : i < n) (ix2 : i < S n) :
+ Vector.nth_order (Vector.shiftout v) ix1 = Vector.nth_order v ix2.
+Proof.
+revert i ix1 ix2.
+elim v using Vector.rectS.
+- lia.
+- intros h n0 t IHv i ix1 ix2.
+  destruct i. 
+  + rewrite !Vector.nth_order_hd.
+    reflexivity.
+  + assert (ix1' : i < n0) by lia.
+    assert (ix2' : i < S n0) by lia.
+    rewrite <-(Vector.nth_order_tl _ _ _ _ ix1').
+    rewrite <-(Vector.nth_order_tl _ _ _ _ ix2').
+    change (VectorDef.nth_order (Vector.shiftout t) ix1' = VectorDef.nth_order t ix2').
+    apply IHv.
+Qed.
+
+Lemma nth_order_append_front {X n m i} (v : Vector.t X n) (w : Vector.t X m) (ix1 : i < n + m) (ix2 : i < n) :
+  Vector.nth_order (v ++ w) ix1 = Vector.nth_order v ix2.
+Proof.
+revert i ix1 ix2.
+induction v;[lia|].
+intros [|i] ix1 ix2;simpl.
+- rewrite !Vector.nth_order_hd.
   reflexivity.
- simpl.
- destruct (Z_lt_le_dec i (two_power_nat i0)) as [Hi0|Hi0]; simpl in *.
-  rewrite testbitToZLo by (rewrite plus_0_r; auto with zarith).
-  apply IHi0; auto with zarith.
- rewrite two_power_nat_S in Hi.
- rewrite testbitToZHi by (rewrite plus_0_r; auto with zarith).
- apply IHi0; rewrite plus_0_r; auto with zarith.
-rewrite <- Hi0; cbn.
-rewrite Nat.eq_add_0 in Hi0.
-destruct Hi0 as [Hi0 Hn].
-rewrite Hi0, Hn.
-change (two_power_nat 0) with 1%Z.
-intros x i Hi.
-replace i with 0%Z by auto with zarith.
+- assert (ix1' : i < n + m) by lia.
+  assert (ix2' : i < n) by lia.
+  rewrite <-(Vector.nth_order_tl _ _ _ _ ix1'), <-(Vector.nth_order_tl _ _ _ _ ix2').
+  simpl.
+  apply IHv.
+Qed.
+
+Lemma nth_order_append_back {X n m i} (v : Vector.t X n) (w : Vector.t X m) (ix1 : n + i < n + m) (ix2 : i < m) :
+  Vector.nth_order (v ++ w) ix1 = Vector.nth_order w ix2.
+Proof.
+revert i ix1 ix2.
+induction v; intros i ix1 ix2.
+- apply Vector.nth_order_ext.
+- simpl.
+  assert (ix1' : n + i < n + m) by lia.
+  rewrite <- (Vector.nth_order_tl _ _ _ _ ix1').
+  apply IHv.
+Qed.
+
+Lemma nth_order_flatten {X n i} (v : Vector (X * X) n) (ix :(i < 2^n)) (ix1 : 2*i < 2^(S n)) (ix2 : 2*i + 1 < 2^(S n)) : 
+         Vector.nth_order (flatten v) ix =
+         (Vector.nth_order (flatten (eq_rect _ tySem v _ (eq_sym VectorPromote))) ix1,
+          Vector.nth_order (flatten (eq_rect _ tySem v _ (eq_sym VectorPromote))) ix2).
+Proof.
+revert v i ix ix1 ix2.
+induction n; intros [v0 v1] i ix ix1 ix2.
+- simpl in *|-.
+  destruct i;[|lia].
+  reflexivity.
+- simpl (@flatten _ (S n) _).
+  simpl (2 ^ _)%nat in *.
+  revert ix.
+  generalize (mul_2_r (2 ^ n)); simpl (2 * 2 ^ n)%nat.
+  intros -> ix.
+  fold (2^n).
+  simpl (eq_rect _ _ _ _ (eq_sym eq_refl)).
+  replace (eq_rect (Vector (X * X) (S n)) tySem (v0, v1) (Vector X (S (S n))) (eq_sym VectorPromote))
+   with ((eq_rect (Vector (X * X) n) tySem v0
+               (Vector X (S n)) (eq_sym VectorPromote)), (eq_rect (Vector (X * X) n) tySem v1
+               (Vector X (S n)) (eq_sym VectorPromote))).
+  2:{
+    generalize (eq_sym (@VectorPromote X (S n))).
+    revert v0 v1.
+    generalize (eq_sym (@VectorPromote X n)).
+    simpl.
+    intros -> v0 v1 e.
+    elim e using K_dec_set;[decide equality|].
+    reflexivity.
+  }
+  set (v0' := (eq_rect (Vector (X * X) n) _ _ _ _)).
+  set (v1' := (eq_rect (Vector (X * X) n) _ _ _ _)).
+  change (@flatten _ (S (S n)) (v0', v1'))
+   with (eq_rect _ (Vector.t X)
+     (flatten v0' ++ flatten v1') _
+     (eq_sym (mul_2_r (2 ^ (S n))))).
+  revert ix1 ix2.
+  generalize (mul_2_r (2 ^ S n)).
+  simpl (2 * _)%nat.
+  simpl (2 ^ _)%nat.
+  intros -> ix1 ix2.
+  change (Vector.nth_order (flatten v0 ++ flatten v1) ix =
+    ( Vector.nth_order (flatten v0' ++ flatten v1') ix1
+    , Vector.nth_order (flatten v0' ++ flatten v1') ix2)).
+  destruct (Nat.le_gt_cases (2^n) i) as [Hi|ix'].
+  + pose (j:= i - 2^n).
+    assert (ix' : j < 2 ^ n) by lia.
+    assert (ix1' : 2 * j < 2 ^ S n) by (cbn; lia).
+    assert (ix2' : 2 * j + 1 < 2 ^ S n) by (cbn; lia).
+    revert ix.
+    pattern i at 1 2.
+    replace i with (2^n + j)%nat by lia.
+    intros ix.
+    fold (2*i)%nat in *.
+    revert ix1.
+    pattern (2*i)%nat at 1 2.
+    replace (2*i)%nat with (2^(S n) + 2*j)%nat by (cbn;lia).
+    intros ix1.
+    revert ix2.
+    replace (2*i + 1)%nat with (2^(S n) + (2*j + 1))%nat by (cbn;lia).
+    intros ix2.
+    rewrite (nth_order_append_back _ _ _ ix'),
+            (nth_order_append_back _ _ _ ix1'),
+            (nth_order_append_back _ _ _ ix2').
+    apply IHn.
+  + assert (ix1' : 2 * i < 2 ^ S n) by (cbn; lia).
+    assert (ix2' : 2 * i + 1 < 2 ^ S n) by (cbn; lia).
+    rewrite (nth_order_append_front _ _ _ ix'),
+            (nth_order_append_front _ _ _ ix1'),
+            (nth_order_append_front _ _ _ ix2').
+    apply IHn.
+Qed.
+
+Lemma nth_order_flatten_if {X n i} (v : Vector (X * X) n) (ix : i < 2^(S n)) (ix_half : Nat.div2 i < 2^n) :
+      Vector.nth_order (flatten (eq_rect _ tySem v _ (eq_sym VectorPromote))) ix =
+      (if Nat.even i then fst else snd) (Vector.nth_order (flatten v) ix_half).
+Proof.
+assert (ix_half1 : 2 * Nat.div2 i < 2 ^ (S n)) by (cbn;lia).
+assert (ix_half2 : 2 * Nat.div2 i + 1 < 2 ^ (S n)) by (cbn;lia).
+rewrite (nth_order_flatten _ _ ix_half1 ix_half2).
+destruct (Nat.Even_Odd_dec i) as [Heven|Hodd].
+- rewrite <- Nat.even_spec in Heven.
+  rewrite Heven.
+  rewrite Nat.even_spec in Heven.
+  destruct Heven as [i' ->].
+  revert ix_half1 ix_half2.
+  rewrite Nat.div2_double.
+  intros; apply Vector.nth_order_ext.
+- rewrite <- Nat.odd_spec in Hodd.
+  rewrite <- Nat.negb_odd, Hodd.
+  rewrite Nat.odd_spec in Hodd.
+  destruct Hodd as [i' ->].
+  revert ix ix_half1 ix_half2.
+  replace (2 * i' + 1)%nat with (S (2 * i'))%nat by lia.
+  rewrite Nat.div2_succ_double.
+  replace (2 * i' + 1)%nat with (S (2 * i'))%nat by lia.
+  intros; apply Vector.nth_order_ext.
+Qed.
+
+Lemma right_shift_const_by_correct {X n v t p i} (ix1 : i < 2^n) (ix2 : i - Pos.to_nat p < 2^n) :
+  Vector.nth_order (@flatten X n (|[ right_shift_const_by t p ]| v)) ix1 =
+  if i <? Pos.to_nat p then |[ t ]| tt else Vector.nth_order (@flatten X n v) ix2.
+Proof.
+revert X t p v i ix1 ix2.
+induction n;intros X t p v i ix1 ix2.
+- simpl in *.
+  destruct i;[|lia].
+  elim (Z.leb_spec);[intros _|lia].
+  elim (Nat.ltb_spec);[intros _|lia].
+  reflexivity.
+- simpl (right_shift_const_by t p v).
+  change (_ <=? _)%Z with  (Zpower_nat 2 (S n) <=? Z.pos p)%Z.
+  elim (Z.leb_spec).
+  1:{
+    rewrite Zpower_nat_Z.
+    change 2%Z with (Z.of_nat 2%nat) at 1.
+    rewrite <- Nat2Z.inj_pow.
+    intros Hp.    
+    elim (Nat.ltb_spec);[intros _|lia].
+    change (Vector.nth_order (flatten (|[@fill _ X (S n)  _ t]| tt)) ix1 = |[t]| tt).
+    rewrite fill_correct.
+    apply nth_replicate.
+  }
+  intros Hpn.
+  transitivity (match p with
+      | (p0~1)%positive => Vector.nth_order (flatten ((
+          eq_rect (Vector (X * X) n)
+            (fun x : Ty => Arrow x x)
+            (right_shift_const_by (t &&& t) p0)
+            (Vector X (S n))
+            (eq_sym VectorPromote)) (right_shift1 t v))) ix1
+      | (p0~0)%positive =>
+          Vector.nth_order (flatten ((eq_rect (Vector (X * X) n)
+            (fun x : Ty => Arrow x x)
+            (right_shift_const_by (t &&& t) p0)
+            (Vector X (S n))
+            (eq_sym VectorPromote)) v)) ix1
+      | 1%positive => Vector.nth_order (flatten (right_shift1 t v)) ix1
+      end);
+  [destruct p; reflexivity|].
+  assert (Hcast : forall (f : Arrow (Vector (X*X) n) (Vector (X*X) n)),
+    (eq_rect _ (fun x : Ty => Arrow x x) f _ (eq_sym VectorPromote) =
+    (fun w => eq_rect _ tySem (f (eq_rect _ tySem w _ VectorPromote)) _ (eq_sym VectorPromote)))).
+  1:{
+    generalize (@VectorPromote X n).
+    intros <-.
+    reflexivity.
+  }
+  assert (ix_half : Nat.div2 i < 2^n).
+  1:{
+    rewrite Nat.div2_div.
+    apply Nat.div_lt_upper_bound;[lia|].
+    rewrite <- Nat.pow_succ_r'.
+    assumption.
+  }
+  specialize (IHn (X*X) (t &&& t)).
+  destruct p.
+  + rewrite Hcast.
+    set (w:= right_shift_const_by (t &&& t) p _).
+    rewrite (nth_order_flatten_if _ _ ix_half).
+    assert (ix_half2 : Nat.div2 i - Pos.to_nat p < 2 ^ n) by lia.
+    rewrite (IHn _ _ _ ix_half ix_half2).
+    elim Nat.ltb_spec; rewrite Nat.div2_div at 1.
+    * intros Hip.
+      elim Nat.ltb_spec.
+      2:{
+        rewrite (Pos2Nat.inj_xI p) at 1.
+        intros Hpi.
+        assert (Hpi0 : S (2 * Pos.to_nat p) / 2 <= i / 2) by (apply Nat.div_le_mono;lia).
+        rewrite <- (Nat.div_unique _ _ (Pos.to_nat p) 1) in Hpi0; lia.
+      }
+      intros _.
+      destruct (Nat.even i);reflexivity.
+    * intros Hpi.
+      assert (ix_half2a : 2*(Nat.div2 i - Pos.to_nat p) < 2 ^ (S n)) by (rewrite Nat.pow_succ_r';lia).
+      assert (ix_half2b : 2*(Nat.div2 i - Pos.to_nat p) + 1 < 2 ^ (S n)) by (rewrite Nat.pow_succ_r';lia).
+      erewrite (nth_order_flatten _ _ ix_half2a ix_half2b).
+      rewrite <-eq_trans_rew_distr, eq_trans_sym_inv_r.
+      cbn -[right_shift1 flatten Pos.to_nat Nat.ltb].
+      rewrite right_shift1_correct.
+      elim Nat.ltb_spec.
+      1:{
+        rewrite (Pos2Nat.inj_xI p) at 1.
+        intros Hip.
+        assert (Hi : (i = 2*Pos.to_nat p)%nat).
+        1:{
+          apply Nat.le_antisymm;[lia|].
+          apply (Nat.mul_le_mono_l _ _ 2) in Hpi.
+          assert (Hle := Nat.mul_div_le i 2).
+          lia.
+        }
+        replace (Nat.even i) with (Nat.even (2 * Pos.to_nat p)%nat) by congruence.
+        rewrite Nat.even_mul.
+        change (Vector.nth_order (Vector.shiftout (t tt :: flatten v)) ix_half2a = t tt).
+        revert ix_half2a.
+        rewrite Hi, Nat.div2_double.
+        replace (2 * (Pos.to_nat p - Pos.to_nat p))%nat with 0 by lia.
+        intros ix_half2a.
+        assert (ix_half2a' : 0 < S (2 ^ S n)) by lia.
+        rewrite (nth_order_shiftout _ _ ix_half2a').
+        rewrite Vector.nth_order_hd.
+        reflexivity.
+      }
+      assert (ix_half2a' : 2 * (Nat.div2 i - Pos.to_nat p) < S (2 ^ S n)) by lia.
+      assert (ix_half2b' : 2 * (Nat.div2 i - Pos.to_nat p) + 1 < S (2 ^ S n)) by lia.
+      rewrite (nth_order_shiftout _ _ ix_half2a'), (nth_order_shiftout _ _ ix_half2b').
+      intros Hp1i.
+      transitivity (Vector.nth_order (Vector.tl (t tt :: flatten v)) ix2);[|reflexivity].
+      assert (ix2' : S (i - Pos.to_nat p~1) < S (2 ^ S n)) by lia.
+      rewrite (VectorSpec.nth_order_tl _ _ _ _ _ ix2').
+      destruct (Nat.Even_Odd_dec i) as [Heven|Hodd].
+      1:{
+        rewrite <- Nat.even_spec in Heven.
+        rewrite Heven.
+        rewrite Nat.even_spec in Heven.
+        destruct Heven as [i' Hi'].
+        revert ix2'.
+        replace (S (i - Pos.to_nat p~1)) with (2 * (Nat.div2 i - Pos.to_nat p))%nat;
+        [intros; apply Vector.nth_order_ext|].
+        rewrite Hi', Nat.div2_double.
+        lia.
+      }
+      1:{
+        rewrite <- Nat.odd_spec in Hodd.
+        rewrite <- Nat.negb_odd, Hodd.
+        rewrite Nat.odd_spec in Hodd.
+        destruct Hodd as [i' Hi'].
+        revert ix2'.
+        replace (S (i - Pos.to_nat p~1)) with (2 * (Nat.div2 i - Pos.to_nat p) + 1)%nat;
+        [intros; apply Vector.nth_order_ext|].
+        replace (2 * i' + 1)%nat with (S (2 * i')) in Hi' by lia.
+        rewrite Hi', Nat.div2_succ_double.
+        lia.
+      }
+  + rewrite Hcast.
+    set (w:= right_shift_const_by (t &&& t) p _).
+    rewrite (nth_order_flatten_if _ _ ix_half).
+    assert (ix_half2 : Nat.div2 i - Pos.to_nat p < 2 ^ n) by lia.
+    rewrite (IHn _ _ _ ix_half ix_half2).
+    elim Nat.ltb_spec; rewrite Nat.div2_div at 1.
+    * intros Hip.
+      elim Nat.ltb_spec.
+      2:{
+        rewrite (Pos2Nat.inj_xO p) at 1.
+        intros Hpi.
+        assert (Hpi0 : (2 * Pos.to_nat p) / 2 <= i / 2) by (apply Nat.div_le_mono;lia).
+        rewrite <- (Nat.div_unique _ _ (Pos.to_nat p) 0) in Hpi0; lia.
+      }
+      intros _.
+      destruct (Nat.even i);reflexivity.
+    * intros Hpi.
+      elim Nat.ltb_spec.
+      1:{ 
+        rewrite (Pos2Nat.inj_xO p) at 1.
+        assert (Hle := Nat.mul_div_le i 2).
+        lia.
+      }
+      assert (ix_half2a : 2*(Nat.div2 i - Pos.to_nat p) < 2 ^ (S n)) by (rewrite Nat.pow_succ_r';lia).
+      assert (ix_half2b : 2*(Nat.div2 i - Pos.to_nat p) + 1 < 2 ^ (S n)) by (rewrite Nat.pow_succ_r';lia).
+      erewrite (nth_order_flatten _ _ ix_half2a ix_half2b).
+      rewrite <-eq_trans_rew_distr, eq_trans_sym_inv_r.
+      cbn -[right_shift1 flatten Pos.to_nat Nat.ltb].
+      intros Hp0i.
+      destruct (Nat.Even_Odd_dec i) as [Heven|Hodd].
+      1:{
+        rewrite <- Nat.even_spec in Heven.
+        rewrite Heven.
+        rewrite Nat.even_spec in Heven.
+        destruct Heven as [i' Hi'].
+        revert ix2.
+        replace (i - Pos.to_nat p~0) with (2 * (Nat.div2 i - Pos.to_nat p))%nat;
+        [intros; apply Vector.nth_order_ext|].
+        rewrite Hi', Nat.div2_double.
+        lia.
+      }
+      1:{
+        rewrite <- Nat.odd_spec in Hodd.
+        rewrite <- Nat.negb_odd, Hodd.
+        rewrite Nat.odd_spec in Hodd.
+        destruct Hodd as [i' Hi'].
+        revert ix2.
+        replace (i - Pos.to_nat p~0) with (2 * (Nat.div2 i - Pos.to_nat p) + 1)%nat;
+        [intros; apply Vector.nth_order_ext|].
+        replace (2 * i' + 1)%nat with (S (2 * i')) in Hi' by lia.
+        rewrite Hi', Nat.div2_succ_double.
+        lia.
+      }
+  + rewrite right_shift1_correct.
+    assert (ix1' : i < S (2 ^ S n)) by lia.
+    rewrite (nth_order_shiftout _ _ ix1').
+    elim Nat.ltb_spec; intros Hi.
+    * destruct i;[|lia].
+      rewrite Vector.nth_order_hd.
+      reflexivity.
+    * destruct i;[lia|].
+      assert (ix1'S : i < 2 ^ S n) by lia.
+      rewrite <- (Vector.nth_order_tl _ _ _ _ ix1'S).
+      change (Vector.nth_order (flatten v) ix1'S = Vector.nth_order (flatten v) ix2).
+      revert ix2.
+      replace (S i - Pos.to_nat 1)%nat with i;
+      [intros; apply Vector.nth_order_ext|lia].
+Qed.
+
+Lemma shiftout_shiftin {X n} a (v : Vector.t X n) : (Vector.shiftout (Vector.shiftin a v)) = v.
+Proof.
+induction v.
+- reflexivity.
+- simpl.
+  rewrite IHv.
+  reflexivity.
+Qed.
+
+Lemma left_shift_const_by_correct {X n v t p i} (ix1 : i < 2^n) :
+  Vector.nth_order (@flatten X n (|[ left_shift_const_by t p ]| v)) ix1 =
+  match lt_dec (i + Pos.to_nat p) (2^n) with
+  | left ix2 => Vector.nth_order (@flatten X n v) ix2
+  | right _ => |[ t ]| tt
+  end.
+Proof.
+revert X t p v i ix1.
+induction n;intros X t p v i ix1.
+- simpl in *.
+  destruct i;[|lia].
+  elim (Z.leb_spec);[intros _|lia].
+  destruct (lt_dec _ _);[lia|reflexivity].
+- simpl (left_shift_const_by t p v).
+  change (_ <=? _)%Z with  (Zpower_nat 2 (S n) <=? Z.pos p)%Z.
+  elim (Z.leb_spec).
+  1:{
+    rewrite Zpower_nat_Z.
+    change 2%Z with (Z.of_nat 2%nat) at 1.
+    rewrite <- Nat2Z.inj_pow.
+    intros Hp.
+    destruct (lt_dec _ _);[lia|].
+    change (Vector.nth_order (flatten (|[@fill _ X (S n)  _ t]| tt)) ix1 = |[t]| tt).
+    rewrite fill_correct.
+    apply nth_replicate.
+  }
+  intros Hpn.
+  transitivity (match p with
+      | (p0~1)%positive => Vector.nth_order (flatten ((
+          eq_rect (Vector (X * X) n)
+            (fun x : Ty => Arrow x x)
+            (left_shift_const_by (t &&& t) p0)
+            (Vector X (S n))
+            (eq_sym VectorPromote)) (left_shift1 t v))) ix1
+      | (p0~0)%positive =>
+          Vector.nth_order (flatten ((eq_rect (Vector (X * X) n)
+            (fun x : Ty => Arrow x x)
+            (left_shift_const_by (t &&& t) p0)
+            (Vector X (S n))
+            (eq_sym VectorPromote)) v)) ix1
+      | 1%positive => Vector.nth_order (flatten (left_shift1 t v)) ix1
+      end);
+  [destruct p; reflexivity|].
+  assert (Hcast : forall (f : Arrow (Vector (X*X) n) (Vector (X*X) n)),
+    (eq_rect _ (fun x : Ty => Arrow x x) f _ (eq_sym VectorPromote) =
+    (fun w => eq_rect _ tySem (f (eq_rect _ tySem w _ VectorPromote)) _ (eq_sym VectorPromote)))).
+  1:{
+    generalize (@VectorPromote X n).
+    intros <-.
+    reflexivity.
+  }
+  assert (ix_half : Nat.div2 i < 2^n).
+  1:{
+    rewrite Nat.div2_div.
+    apply Nat.div_lt_upper_bound;[lia|].
+    rewrite <- Nat.pow_succ_r'.
+    assumption.
+  }
+  specialize (IHn (X*X) (t &&& t)).
+  destruct p.
+  + rewrite Hcast.
+    set (w:= left_shift_const_by (t &&& t) p _).
+    rewrite (nth_order_flatten_if _ _ ix_half).
+    rewrite (IHn _ _ _ ix_half).
+    elim lt_dec; rewrite Nat.div2_div.
+    2:{
+      intros Hip.
+      elim lt_dec.
+      1:{
+        intros Hpi.
+        exfalso.
+        rewrite (Pos2Nat.inj_xI p) in Hpi.
+        rewrite <- Nat.le_succ_l in Hpi.
+        assert (Hpi0 : (i + (S (Pos.to_nat p)) * 2) / 2 <= 2 ^ (S n) / 2) by (apply Nat.div_le_mono;lia).
+        rewrite Nat.div_add in Hpi0 by lia.
+        change (2^(S n)) with (2*(2^n))%nat in Hpi0.
+        rewrite Nat.mul_comm, Nat.div_mul in Hpi0 by lia.
+        lia.
+      }
+      intros _.
+      destruct (Nat.even i);reflexivity.
+    }
+    1:{
+      intros ix_half2.
+      assert (ix_half2a : 2 * (i / 2 + Pos.to_nat p) < 2 ^ (S n)) by (rewrite Nat.pow_succ_r';lia).
+      assert (ix_half2b : 2 * (i / 2 + Pos.to_nat p) + 1 < 2 ^ (S n)) by (rewrite Nat.pow_succ_r';lia).
+      erewrite (nth_order_flatten _ ix_half2 ix_half2a ix_half2b).
+      rewrite <-eq_trans_rew_distr, eq_trans_sym_inv_r.
+      cbn -[left_shift1 flatten Pos.to_nat Nat.ltb].
+      rewrite left_shift1_correct.
+      elim lt_dec.
+      2:{
+        intros Hip.
+        assert (Hi : (i = 2^(S n) - 2*(Pos.to_nat p) - 1)%nat).
+        1:{
+          apply Nat.le_antisymm;[|cbn;lia].
+          apply (Nat.mul_le_mono_l _ _ 2) in ix_half2.
+          assert (Hlt := Nat.mul_succ_div_gt i 2).
+          lia.
+        }
+        replace (Nat.even i) with (Nat.even (2^(S n) - 2*(Pos.to_nat p) - 1)) by congruence.
+        rewrite !Nat.even_sub, Nat.even_pow, Nat.even_mul by lia.
+        change (Vector.nth_order (Vector.tl (Vector.shiftin (t tt) (flatten v))) ix_half2b = t tt).
+        revert ix_half2b.
+        replace (2 * (i / 2 + Pos.to_nat p) + 1)%nat with (pred (2^(S n))).
+        2:{
+          rewrite Nat.mul_add_distr_l, Hi.
+          change (2^ (S n)) with (2*(2^n))%nat.
+          replace (2 * 2 ^ n - 2 * Pos.to_nat p - 1) with (((2 ^ n - Pos.to_nat p -1) * 2 + 1))%nat by lia.
+          rewrite Nat.div_add_l by lia.
+          change (1 / 2) with 0.
+          lia.
+        }
+        intros ix_half2b.
+        assert (ix_half2b' : S (Init.Nat.pred (2 ^ S n)) < S (2 ^ S n)) by lia.
+        rewrite (VectorSpec.nth_order_tl _ _ _ _ _ ix_half2b').
+        revert ix_half2b'.
+        rewrite <- pow_succ.
+        intros ix_half2b'.
+        rewrite Vector.nth_order_last, Vector.shiftin_last.
+        reflexivity.
+      }
+      assert (ix_half2a' : S (2 * (i / 2 + Pos.to_nat p)) < S (2 ^ S n)) by lia.
+      assert (ix_half2b' : S (2 * (i / 2 + Pos.to_nat p) + 1) < S (2 ^ S n)) by lia.
+      rewrite (VectorSpec.nth_order_tl _ _ _ _ _ ix_half2a'),
+              (VectorSpec.nth_order_tl _ _ _ _ _ ix_half2b').
+      intros ix2.
+      transitivity (Vector.nth_order (Vector.shiftout (Vector.shiftin (t tt) (flatten v))) ix2);
+      [|rewrite shiftout_shiftin;reflexivity].
+      assert (ix2' :i + Pos.to_nat p~1 < S (2 ^ n + (2 ^ n + 0))) by lia.
+      rewrite (nth_order_shiftout _ _ ix2').
+      destruct (Nat.Even_Odd_dec i) as [Heven|Hodd].
+      1:{
+        rewrite <- Nat.even_spec in Heven.
+        rewrite Heven.
+        rewrite Nat.even_spec in Heven.
+        destruct Heven as [i' Hi'].
+        revert ix2'.
+        replace (i + Pos.to_nat p~1)%nat with (S (2 * (i / 2 + Pos.to_nat p)))%nat;
+        [intros; apply Vector.nth_order_ext|].
+        rewrite Hi', (Nat.mul_comm _ i'), Nat.div_mul; lia.
+      }
+      1:{
+        rewrite <- Nat.odd_spec in Hodd.
+        rewrite <- Nat.negb_odd, Hodd.
+        rewrite Nat.odd_spec in Hodd.
+        destruct Hodd as [i' Hi'].
+        revert ix2'.
+        replace (i + Pos.to_nat p~1)%nat with (S (2 * (i / 2 + Pos.to_nat p) + 1))%nat;
+        [intros; apply Vector.nth_order_ext|].
+        replace (2 * i' + 1)%nat with (S (2 * i')) in Hi' by lia.
+        rewrite Hi', <- Nat.div2_div, Nat.div2_succ_double.
+        lia.
+      }
+    }
+  + rewrite Hcast.
+    set (w:= left_shift_const_by (t &&& t) p _).
+    rewrite (nth_order_flatten_if _ _ ix_half).
+    rewrite (IHn _ _ _ ix_half).
+    elim lt_dec; rewrite Nat.div2_div.
+    2:{
+      intros Hip.
+      elim lt_dec.
+      1:{
+        intros Hpi.
+        elim Hip.
+        rewrite (Pos2Nat.inj_xO p) in Hpi.
+        change (2^(S n)) with (2*(2^n))%nat in Hpi.
+        assert (Hle := Nat.mul_div_le i 2).
+        cut (i/2 <= 2^n - (Pos.to_nat p + 1));[lia|].
+        apply Nat.div_le_upper_bound;lia.
+      }
+      intros _.
+      destruct (Nat.even i);reflexivity.
+    }
+    1:{
+      intros ix_half2.
+      elim lt_dec.
+      2:{
+        intros Hip.
+        apply Nat.nlt_ge in Hip.
+        rewrite (Pos2Nat.inj_xO p) in Hip.
+        apply (Nat.div_le_mono _ _ 2) in Hip;[|lia].
+        change (2^(S n)) with (2*(2^n))%nat in Hip.
+        rewrite Nat.mul_comm, Nat.div_mul in Hip by lia.
+        rewrite Nat.mul_comm, Nat.div_add in Hip by lia.
+        lia.
+      }
+      assert (ix_half2a : 2 * (i / 2 + Pos.to_nat p) < 2 ^ S n) by (rewrite Nat.pow_succ_r';lia).
+      assert (ix_half2b : 2 * (i / 2 + Pos.to_nat p) + 1 < 2 ^ S n) by (rewrite Nat.pow_succ_r';lia).
+      erewrite (nth_order_flatten _ _ ix_half2a ix_half2b).
+      rewrite <-eq_trans_rew_distr, eq_trans_sym_inv_r.
+      cbn -[flatten Pos.to_nat Nat.ltb].
+      intros ix2.
+      destruct (Nat.Even_Odd_dec i) as [Heven|Hodd].
+      1:{
+        rewrite <- Nat.even_spec in Heven.
+        rewrite Heven.
+        rewrite Nat.even_spec in Heven.
+        destruct Heven as [i' Hi'].
+        revert ix2.
+        replace (i + Pos.to_nat p~0)%nat with (2 * (i / 2 + Pos.to_nat p))%nat;
+        [intros; apply Vector.nth_order_ext|].
+        rewrite Hi', <- Nat.div2_div, Nat.div2_double.
+        lia.
+      }
+      1:{
+        rewrite <- Nat.odd_spec in Hodd.
+        rewrite <- Nat.negb_odd, Hodd.
+        rewrite Nat.odd_spec in Hodd.
+        destruct Hodd as [i' Hi'].
+        revert ix2.
+        replace (i + Pos.to_nat p~0)%nat with (2 * (i / 2 + Pos.to_nat p) + 1)%nat;
+        [intros; apply Vector.nth_order_ext|].
+        replace (2 * i' + 1)%nat with (S (2 * i')) in Hi' by lia.
+        rewrite Hi', <- Nat.div2_div, Nat.div2_succ_double.
+        lia.
+      }
+    }
+  + rewrite left_shift1_correct.
+    assert (ix1' : S i < S (2 ^ S n)) by lia.
+    rewrite (Vector.nth_order_tl _ _ _ _ _ ix1').
+    elim lt_dec; intros Hi.
+    * transitivity (VectorDef.nth_order (Vector.shiftout (Vector.shiftin (t tt) (flatten v))) Hi).
+      1:{
+       revert Hi.
+       replace (i + Pos.to_nat 1)%nat with (S i) by lia.
+       intros Hi.
+       rewrite (nth_order_shiftout _ _ ix1').
+       reflexivity.
+      }
+      f_equal.
+      apply shiftout_shiftin.
+    * revert ix1'.
+      replace (S i) with (2^S n) by lia.
+      intros ix1'.
+      rewrite Vector.nth_order_last.
+      apply Vector.shiftin_last.
+Qed.
+
+Lemma nth_Word {n i} (x : Word n) (ix : i < 2^n) :
+  toBool (Vector.nth_order (flatten x) ix) = Z.testbit (toZ x) (2^(Z.of_nat n) - 1 - Z.of_nat i).
+Proof.
+revert i x ix.
+induction n.
+- intros [|i];[|cbn;lia].
+  intros [[] | []];reflexivity.
+- intros i [x0 x1].
+  rewrite <- (Nat2Z.inj_pow 2) in *.
+  simpl.
+  generalize (mul_2_r (2 ^ n)); simpl.
+  intros -> ix; simpl.
+  destruct (lt_dec i (2^n)) as [ix'|Hi].
+  + rewrite (nth_order_append_front _ _ _ ix'), IHn, testbitToZHi;
+    rewrite two_power_nat_equiv, <- (Nat2Z.inj_pow 2);[f_equal|];lia.
+  + assert (ix' : i - 2^n < 2^n) by lia.
+    revert ix.
+    replace i with (2^n + (i - 2^n))%nat by lia.
+    intros ix.
+    rewrite (nth_order_append_back _ _ _ ix'), IHn, testbitToZLo;[f_equal;lia|].
+    rewrite two_power_nat_equiv, <- (Nat2Z.inj_pow 2).
+    lia.
+Qed.
+
+Lemma shift_const_correct n z (x : Word n) i (Hi : (0 <= i < two_power_nat n)%Z) :
+  Z.testbit (toZ (|[shift_const (-z)]| x : tySem (Word n))) i = Z.testbit (toZ x) (i + z)%Z.
+Proof.
+assert (Htwo : forall n, two_power_nat n = Z.of_nat (2 ^ n)).
+1:{
+  intros.
+  rewrite two_power_nat_equiv, <- (Nat2Z.inj_pow 2).
+  reflexivity.
+}
+rewrite Htwo in *.
+assert (ix : 2^n - 1 - Z.to_nat i < 2^n) by lia.
+destruct z;cbn.
+- f_equal.
+  lia.
+- replace i with (Z.of_nat (2 ^  n - 1 - (2 ^ n - 1 - Z.to_nat i))) at 1 by lia.
+  rewrite Nat2Z.inj_sub, (Nat2Z.inj_sub _ 1), Nat2Z.inj_pow by lia.
+  rewrite <- (nth_Word _ ix).
+  assert (ix2 : (2 ^ n - 1 - Z.to_nat i) - Pos.to_nat p < 2 ^ n) by lia.
+  rewrite (right_shift_const_by_correct _ ix2).
+  elim Nat.ltb_spec; intros Hp.
+  + rewrite toZ_mod.
+    rewrite two_power_nat_equiv, Z.mod_pow2_bits_high;[reflexivity|].
+    rewrite bitSize_Word, two_power_nat_equiv, <- (Nat2Z.inj_pow 2). lia.
+  + rewrite nth_Word.
+    f_equal.
+    rewrite <- (Nat2Z.inj_pow 2).
+    lia.
+- replace i with (Z.of_nat (2 ^  n - 1 - (2 ^ n - 1 - Z.to_nat i))) at 1 by lia.
+  rewrite Nat2Z.inj_sub, (Nat2Z.inj_sub _ 1), Nat2Z.inj_pow by lia.
+  rewrite <- (nth_Word _ ix).
+  rewrite left_shift_const_by_correct.
+  elim lt_dec; intros Hp.
+  + rewrite nth_Word.
+    f_equal.
+    rewrite <- (Nat2Z.inj_pow 2).
+    lia.
+  + rewrite Z.testbit_neg_r;[reflexivity|].
+    lia.
+Qed.
+
+Lemma left_rotate1_correct {X n v} :
+  @flatten X n (|[ left_rotate1 ]| v) = Vector.tl (Vector.shiftin (pow_hd (flatten v)) (flatten v)).
+Proof.
+unfold left_rotate1.
+etransitivity;[cbn|reflexivity].
+change (flatten (snd _)) with (snd (map_snd flatten (|[full_left_shift1]| (v, |[leftmost]| v)))).
+rewrite full_left_shift1_correct, leftmost_correct.
 reflexivity.
 Qed.
 
-Lemma subseqWrapPair_correct n m z rec (Hrec : forall m z, subseqWrapSpec n m z (rec m z)) :
-  subseqWrapSpec (S n) m z (subseqWrapPair z rec).
+Lemma right_rotate1_correct {X n v} :
+  @flatten X n (|[ right_rotate1 ]| v) = Vector.shiftout (pow_last (flatten v) :: (flatten v)).
 Proof.
-assert (Hpos : (0 < two_power_nat (S n))%Z).
- rewrite two_power_nat_equiv; auto using Z.pow_pos_nonneg with zarith.
-assert (Hlt : (two_power_nat n <= two_power_nat (S n))%Z)
- by auto using two_power_nat_le with arith.
-intros x i Hi.
-rewrite <- Zplus_mod_idemp_r.
-revert z x i Hi; induction m; intros z [xhi xlo] i Hi; cbn -[toZ zero subseqWrap0 Word];
- assert (Hz' := Z.mod_pos_bound z (two_power_nat (S n)) Hpos); 
- set (z':=Zmod z (two_power_nat (S n))) in *;
-(destruct Z.eq_dec as [->|];[apply subseqWrap0_correct; auto|]);
- repeat destruct Z_lt_le_dec; simpl;
- change (two_power_nat 0) with 1%Z in *;
- solve
- [rewrite Z.mod_small, Hrec, testbitToZLo, Z.mod_small; auto with zarith
- |rewrite Z.mod_small, Hrec, testbitToZHi, <- Z.add_sub_assoc, Z.mod_small;
-   repeat rewrite two_power_nat_S in *; auto with zarith
- |destruct (Z_lt_le_dec i (two_power_nat m)) as [Hi0|Hi0];
-  [rewrite (testbitToZLo _ _ Hi0), IHm, Zplus_mod_idemp_r; auto with zarith
-  |repeat rewrite two_power_nat_S in *; rewrite (testbitToZHi _ _ Hi0), IHm, Zplus_mod_idemp_r by auto with zarith
-  ]; do 2 f_equal; ring
- ].
+unfold right_rotate1.
+etransitivity;[cbn|reflexivity].
+change (flatten (fst _)) with (fst (map_fst flatten (|[full_right_shift1]| (|[rightmost]| v, v)))).
+rewrite full_right_shift1_correct, rightmost_correct.
+reflexivity.
 Qed.
 
-Lemma subseqWrap_correct n : forall m z, subseqWrapSpec n m z (subseqWrap z).
+Lemma foldr_comp_correct {X} l v : |[foldr_comp l]| v = fold_right (@comp X X X CoreFunSem) |[iden]| l v.
 Proof.
-induction n; intros; cbn -[subseqWrap0];
-auto using subseqWrapBit_correct, subseqWrapPair_correct.
+revert v.
+induction l;[reflexivity|].
+destruct l as [|b l];[reflexivity|].
+- intros v. 
+  change (foldr_comp (a :: b :: l) v) with (foldr_comp (b :: l) (a v)).
+  apply IHl.
 Qed.
 
-Lemma rotate_correct n z (x : Word n) i (Hi : (0 <= i < two_power_nat n)%Z) :
-  Z.testbit (toZ (|[rotate z]| x)) i = Z.testbit (toZ x) (Zmod (i + z) (two_power_nat n))%Z.
+Lemma rotate_const_correct {X n i j} z (v : Vector X n) (ix : i < 2^n) (jx : j < 2^n) :
+  eqm (2^Z.of_nat n) (Z.of_nat j) (Z.of_nat i + z) ->
+  Vector.nth_order (flatten (|[rotate_const z]| v)) ix = Vector.nth_order (flatten v) jx.
 Proof.
-exact (subseqWrap_correct n z x Hi).
+rewrite <- (Nat2Z.inj_pow 2).
+unfold rotate_const.
+rewrite foldr_comp_correct.
+intros Hij.
+generalize jx.
+rewrite <-(Nat2Z.id j), <-(Z.mod_small (Z.of_nat j) (Z.of_nat (2^n))), Hij by lia.
+clear j jx Hij.
+intros jx.
+assert (ixmod : forall n a, Z.to_nat (a  mod Z.of_nat (2 ^ n)) < 2 ^ n).
+1:{
+  clear.
+  intros n a.
+  assert (Hmod := Z.mod_pos_bound a (Z.of_nat (2^n))).
+  rewrite pow_succ in Hmod at 1.
+  lia.
+}
+transitivity (Vector.nth_order (flatten v) (ixmod _ (Z.of_nat i + z)))%Z;[|apply Vector.nth_order_ext].
+clear jx.
+revert X i z v ix.
+induction n;
+[intros X [|i] z;simpl;[generalize (ixmod 0 z);simpl;rewrite Z.mod_1_r;intros;apply Vector.nth_order_ext|lia] |].
+intros X i z v ix.
+assert (Hcast : forall (l : list (Arrow (Vector (X*X) n) (Vector (X*X) n))) w,
+  fold_right comp iden (eq_rect _ (fun x : Ty => list (Arrow x x)) l _ (eq_sym VectorPromote)) w =
+  eq_rect _ tySem (fold_right comp iden l (eq_rect _ tySem w _ VectorPromote)) _ (eq_sym VectorPromote)).
+1:{
+  generalize (@VectorPromote X n).
+  intros <-.
+  reflexivity.
+}
+assert (ix_half : Nat.div2 i < 2^n).
+1:{
+  rewrite Nat.div2_div.
+  apply Nat.div_lt_upper_bound;[lia|].
+  rewrite <- Nat.pow_succ_r'.
+  assumption.
+}
+assert (Heven : forall a, Nat.even a = Z.even (Z.of_nat a)).
+1:{
+  clear.
+  intros a.
+  induction a as [a IH] using lt_wf_ind.
+  destruct a as [| [|a]]; try reflexivity.
+  simpl (Nat.even _).
+  rewrite IH;[|lia].
+  symmetry.
+  etransitivity;[|apply Z.even_succ_succ].
+  f_equal.
+  lia.
+}
+generalize (ixmod (S n) (Z.of_nat i + z)%Z).
+change (2^S n) with (2 * 2^n)%nat.
+rewrite Nat2Z.inj_mul.
+change (Z.of_nat 2) with 2%Z.
+intros jx.
+simpl (rotate_const_list z).
+case_eq (Z.even z);[|case_eq (Z.even (z/2))].
+- rewrite Z.even_spec.
+  intros [z' ->].
+  replace (2 * z' / 2)%Z with z' by (rewrite Z.mul_comm, Z_div_mult by lia;reflexivity).
+  rewrite Hcast, (nth_order_flatten_if _ _ ix_half).
+  rewrite (IHn _ _ _ _ ix_half).
+  generalize (ixmod n (Z.of_nat (Nat.div2 i) + z')%Z).
+  set (j := Z.to_nat
+       ((Z.of_nat i + 2 * z') mod (2 * Z.of_nat (2 ^ n)))) in *.
+  replace (Z.to_nat ((Z.of_nat (Nat.div2 i) + z') mod Z.of_nat (2 ^ n))) 
+     with (Nat.div2 j).
+  2:{
+    symmetry.
+    rewrite !Nat.div2_div, Nat2Z.inj_div, <- Z_div_plus, <-Zaux.Zdiv_mod_mult, Z.mul_comm by lia.
+    rewrite Z2Nat.inj_div by (assert (Hmod := Z.mod_pos_bound (Z.of_nat i + Z.of_nat 2 * z') (Z.of_nat 2 * Z.of_nat (2 ^ n)));lia). 
+    reflexivity.
+  }
+  intros jx_half.
+  replace (Nat.even i) with (Nat.even j);
+  [rewrite <-(nth_order_flatten_if _ jx jx_half), <-eq_trans_rew_distr, eq_trans_sym_inv_r;
+   apply Vector.nth_order_ext|].
+  rewrite !Heven.
+  symmetry.
+  apply Bool.eqb_true_iff.
+  rewrite <- Z.even_sub.
+  symmetry.
+  change ((Z.even 2 || Z.even z') = Z.even (Z.of_nat i - Z.of_nat j))%bool.
+  apply Bool.eqb_true_iff.
+  rewrite <- Z.even_mul, <- Z.even_add, Zeven_mod.
+  apply Zeq_is_eq_bool.
+  replace (_ + _)%Z with ((Z.of_nat i + 2 * z') - Z.of_nat j)%Z by lia.
+  apply Z.mod_divide;[lia|].
+  etransitivity;[apply (Z.divide_factor_l 2 (Z.of_nat (2^n)))|].
+  apply Z.mod_divide;[lia|].
+  unfold j.
+  rewrite Z2Nat.id by (assert (Hmod := Z.mod_pos_bound (Z.of_nat i + 2 * z') (2 * Z.of_nat (2^n)));lia).
+  rewrite Zminus_mod_idemp_r, Z.sub_diag.
+  reflexivity.
+- rewrite Z.even_spec, <-Z.negb_odd, Bool.negb_false_iff, Z.odd_spec.
+  intros Hz' [z' ->].
+  replace ((2 * z' + 1) / 2)%Z with z' in * by (rewrite Z.mul_comm, Z.div_add_l, Z.add_0_r by lia;reflexivity).
+  destruct Hz' as [z ->].
+  set (l := eq_rect _ _ _ _ _).
+  change (fold_right comp H (_ :: l) v) with (fold_right comp H l (|[left_rotate1]| v)).
+  rewrite Hcast, (nth_order_flatten_if _ _ ix_half), (IHn _ _ _ _ ix_half); clear l.
+  generalize (ixmod n (Z.of_nat (Nat.div2 i) + 2 * z)%Z).  
+  rewrite Nat.div2_div, Nat2Z.inj_div, <- Z_div_plus, <-Zaux.Zdiv_mod_mult, Z.mul_comm by lia.
+  change (Z.of_nat 2) with 2%Z.
+  set (k:= (Z.of_nat i + 2 * (2 * z))%Z).
+  assert (Hmod := Z.mod_pos_bound k (2 * Z.of_nat (2^n))).
+  rewrite Z2Nat.inj_div by lia.
+  rewrite <-Nat.div2_div.
+  revert jx.
+  rewrite Z.add_assoc.
+  set (j := Z.to_nat (k mod (2 * Z.of_nat (2 ^ n)))).
+  intros jx jx_half.
+  assert (jx' : j < 2 ^ (S n)) by (cbn;lia).
+  replace (Nat.even i) with (Nat.even j).
+  * rewrite <-(nth_order_flatten_if _ jx'), <-eq_trans_rew_distr, eq_trans_sym_inv_r;
+    simpl (eq_rect _ _ _ _ eq_refl).
+    rewrite left_rotate1_correct.
+    assert (jx'S : S j < S (2^S n)) by lia.
+    rewrite (VectorSpec.nth_order_tl _ _ _ _ _ jx'S).
+    elim (lt_dec (S j) (2 ^ S n)).
+    + intros jx'S'.
+      rewrite <- (nth_order_shiftout _ jx'S'), shiftout_shiftin.
+      revert jx.
+      fold k.
+      rewrite <- Zplus_mod_idemp_l, Z.mod_small;
+      [rewrite Z2Nat.inj_succ;[apply Vector.nth_order_ext|lia] |].
+      unfold j in jx'S'.
+      rewrite <- Z2Nat.inj_succ in jx'S' by lia.
+      change (2^S n) with (2 * 2^n)%nat in *.
+      lia.
+    + intros Hj.
+      revert jx'S.
+      replace (S j) with (2 ^ S n) by lia.
+      intros jx'S.
+      rewrite Vector.nth_order_last, Vector.shiftin_last.
+      revert jx.
+      rewrite <-Zplus_mod_idemp_l, <-(Z2Nat.id (k mod (2 * Z.of_nat (2 ^ n)))) by lia.
+      fold (Z.succ (Z.of_nat (Z.to_nat (k mod (2 * Z.of_nat (2 ^ n)))))) j.
+      rewrite <- Nat2Z.inj_succ.
+      replace (S j) with (2 ^ S n) by lia.
+      change (2^S n) with (2 * 2^n)%nat.
+      rewrite Nat2Z.inj_mul, Z_mod_same_full.
+      change (2 * 2^n)%nat with (2^S n).
+      generalize (flatten v).
+      unfold pow_hd.
+      generalize (pow_succ (S n));intros -> w wx.
+      symmetry.
+      apply Vector.nth_order_hd.
+  * rewrite !Heven, !Zeven_mod.
+    change 2%Z with (2^1)%Z.
+    unfold j.
+    rewrite Z2Nat.id, Nat2Z.inj_pow, <- Z.pow_succ_r, <- !Z.land_ones, <- Z.land_assoc by lia.
+    rewrite Z.land_ones, Z.ones_mod_pow2, !Z.land_ones, <-!Zeven_mod by lia.
+    unfold k.
+    rewrite Z.even_add, Z.even_mul.
+    change (_ || _)%bool with (Z.even 0).
+    rewrite <-Z.even_add.
+    f_equal.
+    lia.
+- rewrite <-!Z.negb_odd, !Bool.negb_false_iff, !Z.odd_spec.
+  intros Hz' [z' ->].
+  replace ((2 * z' + 1) / 2)%Z with z' in * by (rewrite Z.mul_comm, Z.div_add_l, Z.add_0_r by lia;reflexivity).
+  destruct Hz' as [z ->].
+  replace (2 * (2 * z + 1) + 1 + 1)%Z with ((2*(z + 1))*2)%Z by lia.
+  rewrite Z_div_mult by lia.
+  set (l := eq_rect _ _ _ _ _).
+  change (fold_right comp H (_ :: l) v) with (fold_right comp H l (|[right_rotate1]| v)).
+  rewrite Hcast, (nth_order_flatten_if _ _ ix_half), (IHn _ _ _ _ ix_half); clear l.
+  generalize (ixmod n (Z.of_nat (Nat.div2 i) + 2 * (z + 1))%Z).  
+  rewrite Nat.div2_div, Nat2Z.inj_div, <- Z_div_plus, <-Zaux.Zdiv_mod_mult, Z.mul_comm by lia.
+  change (Z.of_nat 2) with 2%Z.
+  set (k:= (Z.of_nat i + 2 * (2 * (z + 1)))%Z).
+  assert (Hmod := Z.mod_pos_bound k (2 * Z.of_nat (2^n))).
+  rewrite Z2Nat.inj_div by lia.
+  rewrite <-Nat.div2_div.
+  revert jx.
+  replace (Z.of_nat i + (2 * (2 * z + 1) + 1))%Z with (k - 1)%Z by lia.
+  set (j := Z.to_nat (k mod (2 * Z.of_nat (2 ^ n)))).
+  intros jx jx_half.
+  assert (jx' : j < 2 ^ (S n)) by (cbn;lia).
+  replace (Nat.even i) with (Nat.even j).
+  * rewrite <-(nth_order_flatten_if _ jx'), <-eq_trans_rew_distr, eq_trans_sym_inv_r;
+    simpl (eq_rect _ _ _ _ eq_refl).
+    rewrite right_rotate1_correct.
+    assert (jx'S : j < S (2^S n)) by lia.
+    rewrite (nth_order_shiftout _ _ jx'S).
+    elim (Nat.eq_dec j 0).
+    + intros Hj.
+      revert jx'S.
+      rewrite Hj.
+      intros jx'S.
+      rewrite Vector.nth_order_hd.
+      revert jx.
+      rewrite <-Zplus_mod_idemp_l, <-(Z2Nat.id (k mod (2 * Z.of_nat (2 ^ n)))) by lia.
+      fold j.
+      rewrite Hj.
+      simpl (Z.of_nat 0).
+      rewrite <- (Z_mod_same_full (2 * Z.of_nat (2 ^ n))), Zplus_mod_idemp_l, Z.mod_small by lia.
+      replace (_ * _)%Z with (Z.of_nat (2 * 2 ^ n)) by lia.
+      change (2 * 2^n)%nat with (2^S n).
+      generalize (flatten v).
+      unfold pow_last.
+      generalize (pow_succ (S n));intros -> w.
+      replace (Z.to_nat _) with (Init.Nat.pred (2 ^ S n)) by lia.
+      intros wx.
+      symmetry.
+      apply Vector.nth_order_last.
+    + intros Hj.
+      revert jx'S.
+      replace j with (S (pred j)) by lia.
+      intros jx'S.
+      symmetry.
+      change (flatten v) with (Vector.tl (pow_last (flatten v) :: flatten v)) at 1.
+      revert jx.
+      rewrite <-Zplus_mod_idemp_l, <-(Z2Nat.id (k mod (2 * Z.of_nat (2 ^ n)))) by lia.
+      fold j.
+      replace (Z.of_nat j + - (1))%Z with (Z.of_nat (pred j)) by lia.
+      rewrite Z.mod_small, Nat2Z.id by lia.
+      change (2 * 2^n)%nat with (2^S n).
+      intros jx.
+      apply Vector.nth_order_tl.
+  * rewrite !Heven, !Zeven_mod.
+    change 2%Z with (2^1)%Z.
+    unfold j.
+    rewrite Z2Nat.id, Nat2Z.inj_pow, <- Z.pow_succ_r, <- !Z.land_ones, <- Z.land_assoc by lia.
+    rewrite Z.land_ones, Z.ones_mod_pow2, !Z.land_ones, <-!Zeven_mod by lia.
+    unfold k.
+    rewrite Z.even_add, Z.even_mul.
+    change (_ || _)%bool with (Z.even 0).
+    rewrite <-Z.even_add.
+    f_equal.
+    lia.
+Qed.
+
+Lemma rotate_const_correct_word n z (x : Word n) i (Hi : (0 <= i < two_power_nat n)%Z) :
+  Z.testbit (toZ (|[rotate_const (-z)]| x : tySem (Word n))) i = Z.testbit (toZ x) (Zmod (i + z) (two_power_nat n))%Z.
+Proof.
+assert (Htwo : forall n, two_power_nat n = Z.of_nat (2 ^ n)).
+1:{
+  intros.
+  rewrite two_power_nat_equiv, <- (Nat2Z.inj_pow 2).
+  reflexivity.
+}
+rewrite Htwo in *.
+set (i0 := Z.to_nat (Z.of_nat (2^n) - 1 - i)).
+assert (ix : i0 < 2^n) by lia.
+replace i with (Z.of_nat (2 ^ n) - 1 - Z.of_nat i0)%Z at 1 by lia.
+rewrite Nat2Z.inj_pow by lia.
+rewrite <- (nth_Word _ ix).
+set (j0 := Z.to_nat ((Z.of_nat (2^n) - 1 - i - z) mod (2^Z.of_nat n))).
+destruct (Z.mod_pos_bound (Z.of_nat (2 ^ n) - 1 - i - z) (2 ^ Z.of_nat n)) as [Hj0 Hj1];[lia|].
+assert (jx : j0 < 2^n).
+1:{
+  rewrite <- (Nat2Z.id (2^n)).
+  rewrite Nat2Z.inj_pow by lia.
+  apply Z2Nat.inj_lt;lia.
+}
+rewrite (rotate_const_correct _ _ _ jx).
+2:{
+  unfold eqm, i0, j0.
+  rewrite !Z2Nat.id, Zmod_mod by lia.
+  reflexivity.
+}
+rewrite nth_Word.
+f_equal.
+rewrite <-(Z.mod_small (2 ^ Z.of_nat n - 1 - Z.of_nat j0)%Z (2 ^ Z.of_nat n)) by lia.
+unfold j0.
+rewrite Z2Nat.id, Nat2Z.inj_pow, Zminus_mod_idemp_r by lia.
+f_equal.
+lia.
 Qed.
 
 End Specifications.
 
 Lemma zero_Parametric {n} {term1 term2 : Core.Algebra} (R : Core.Parametric.Rel term1 term2) : R _ (Word n) zero zero.
 Proof.
-induction n; simpl; auto with parametricity.
+induction n; cbn; auto with parametricity.
 Qed.
 Hint Immediate zero_Parametric : parametricity.
 
@@ -794,14 +1970,14 @@ Hint Resolve buildFullAdder_Parametric : parametricity.
 Lemma fullAdder_Parametric {term1 term2 : Core.Algebra} (R : Core.Parametric.Rel term1 term2)
   {n} : R _ _ fullAdder (@fullAdder n _).
 Proof.
-induction n; simpl; auto with parametricity.
+induction n; cbn; auto with parametricity.
 Qed.
 Hint Immediate fullAdder_Parametric : parametricity.
 
 Lemma adder_Parametric {term1 term2 : Core.Algebra} (R : Core.Parametric.Rel term1 term2)
   {n} : R _ _ adder (@adder n _).
 Proof.
-induction n; simpl; auto with parametricity.
+induction n; cbn; auto with parametricity.
 Qed.
 Hint Immediate adder_Parametric : parametricity.
 
@@ -823,7 +1999,7 @@ Hint Resolve buildFullMultiplier_Parametric : parametricity.
 Lemma fullMultiplier_Parametric {term1 term2 : Core.Algebra} (R : Core.Parametric.Rel term1 term2)
   {n} : R _ (Word n * Word n) fullMultiplier (@fullMultiplier n _).
 Proof.
-induction n; simpl; auto with parametricity.
+induction n; cbn; auto with parametricity.
 Qed.
 Hint Immediate fullMultiplier_Parametric : parametricity.
 
@@ -831,9 +2007,24 @@ Lemma multiplier_Parametric {term1 term2 : Core.Algebra} (R : Core.Parametric.Re
   {n} : R _ _ multiplier (@multiplier n _).
 Proof.
 unfold multiplier.
-simpl; auto with parametricity.
+cbn; auto with parametricity.
 Qed.
 Hint Immediate multiplier_Parametric : parametricity.
+
+Lemma build_fill_Parametric {term1 term2 : Core.Algebra} (R : Core.Parametric.Rel term1 term2)
+  {C X} t1 t2 : R C X t1 t2 -> R _ _ (build_fill t1) (build_fill t2).
+Proof.
+unfold build_fill.
+auto 10 with parametricity.
+Qed.
+Hint Resolve build_fill_Parametric : parametricity.
+
+Lemma fill_Parametric {term1 term2 : Core.Algebra} (R : Core.Parametric.Rel term1 term2)
+  {C X n} op1 op2 : R _ _ op1 op2 -> R _ _ (fill op1) (@fill C X n _ op2).
+Proof.
+induction n; simpl; auto with parametricity.
+Qed.
+Hint Resolve fill_Parametric : parametricity.
 
 Lemma buildBitwiseTri_Parametric {term1 term2 : Core.Algebra} (R : Core.Parametric.Rel term1 term2)
   {W} t1 t2 : R _ W t1 t2 -> R _ _ (buildBitwiseTri t1) (buildBitwiseTri t2).
@@ -844,96 +2035,191 @@ Qed.
 Hint Resolve buildBitwiseTri_Parametric : parametricity.
 
 Lemma bitwiseTri_Parametric {term1 term2 : Core.Algebra} (R : Core.Parametric.Rel term1 term2)
-  {n} op1 op2 : R _ _ op1 op2 -> R _ _ (bitwiseTri op1) (@bitwiseTri n _ op2).
+  {X n} op1 op2 : R _ _ op1 op2 -> R _ _ (bitwiseTri op1) (@bitwiseTri X n _ op2).
 Proof.
 induction n; simpl; auto with parametricity.
 Qed.
 Hint Resolve bitwiseTri_Parametric : parametricity.
 
-Lemma subseq0_Parametric {n m} {term1 term2 : Core.Algebra} (R : Core.Parametric.Rel term1 term2) :
-  R (Word n) (Word m) subseq0 subseq0.
+Lemma build_leftmost_Parametric {term1 term2 : Core.Algebra} (R : Core.Parametric.Rel term1 term2)
+  {V X} t1 t2 : R V X t1 t2 -> R _ _ (build_leftmost t1) (build_leftmost t2).
 Proof.
-unfold subseq0.
-destruct (natDiff n m) as [[i []] | [i []]];
- induction i; cbn; auto with parametricity.
+unfold build_leftmost.
+auto 10 with parametricity.
 Qed.
-Hint Immediate subseq0_Parametric : parametricity.
+Hint Resolve build_leftmost_Parametric : parametricity.
 
-Lemma subseqBit_Parametric {n} z {term1 term2 : Core.Algebra} (R : Core.Parametric.Rel term1 term2) :
-  R _ (Word n) (subseqBit z) (subseqBit z).
+Lemma leftmost_Parametric {term1 term2 : Core.Algebra} (R : Core.Parametric.Rel term1 term2)
+  {X n} : R _ _ leftmost (@leftmost X n term2).
 Proof.
-revert z; induction n; cbn; intros z;
-[destruct (Z.eq_dec _ _)|]; auto with parametricity.
+induction n; simpl; auto with parametricity.
 Qed.
-Hint Immediate subseqBit_Parametric : parametricity.
+Hint Resolve leftmost_Parametric : parametricity.
 
-Lemma subseqPair_Parametric {n m} z {term1 term2 : Core.Algebra} rec1 rec2 (R : Core.Parametric.Rel term1 term2) :
-  (forall m z, R (Word n) (Word m) (rec1 m z) (rec2 m z)) ->
-  R (Word n * Word n) (Word m) (subseqPair z rec1) (subseqPair z rec2).
+Lemma build_rightmost_Parametric {term1 term2 : Core.Algebra} (R : Core.Parametric.Rel term1 term2)
+  {V X} t1 t2 : R V X t1 t2 -> R _ _ (build_rightmost t1) (build_rightmost t2).
 Proof.
-change (R (Word n * Word n)) with (R (Word (S n))).
-revert z; induction m; simpl subseqPair; intros z Hrec;
-destruct (Z.eq_dec _ _) as [|];
-repeat destruct Z_lt_le_dec;
-repeat first [apply pair_Parametric
-             |refine (drop_Parametric _ _ _ _)
-             |refine (take_Parametric _ _ _ _)
-             |destruct Zlt_not_le];
-auto with parametricity.
+unfold build_rightmost.
+auto 10 with parametricity.
 Qed.
-Hint Resolve subseqPair_Parametric : parametricity.
+Hint Resolve build_rightmost_Parametric : parametricity.
 
-Lemma subseq_Parametric {n m} z {term1 term2 : Core.Algebra} (R : Core.Parametric.Rel term1 term2) :
-  R (Word n) (Word m) (subseq z) (subseq z).
+Lemma rightmost_Parametric {term1 term2 : Core.Algebra} (R : Core.Parametric.Rel term1 term2)
+  {X n} : R _ _ rightmost (@rightmost X n term2).
 Proof.
-revert m z; induction n; simpl; auto with parametricity.
+induction n; simpl; auto with parametricity.
 Qed.
-Hint Immediate subseq_Parametric : parametricity.
+Hint Resolve rightmost_Parametric : parametricity.
 
-Lemma shift_Parametric {n} z {term1 term2 : Core.Algebra} (R : Core.Parametric.Rel term1 term2) :
-  R (Word n) (Word n) (shift z) (shift z).
+Lemma build_full_left_shift1_Parametric {term1 term2 : Core.Algebra} (R : Core.Parametric.Rel term1 term2)
+  {X W} t1 t2 : R (W * X) (X * W) t1 t2 -> R _ _ (build_full_left_shift1 t1) (build_full_left_shift1 t2).
 Proof.
-unfold shift.
-auto with parametricity.
+unfold build_full_left_shift1.
+auto 10 with parametricity.
 Qed.
-Hint Immediate shift_Parametric : parametricity.
+Hint Resolve build_full_left_shift1_Parametric : parametricity.
 
-Lemma subseqWrap0_Parametric {n m} {term1 term2 : Core.Algebra} (R : Core.Parametric.Rel term1 term2) :
-  R (Word n) (Word m) subseqWrap0 subseqWrap0.
+Lemma full_left_shift1_Parametric {term1 term2 : Core.Algebra} (R : Core.Parametric.Rel term1 term2)
+  {X n} : R _ _ full_left_shift1 (@full_left_shift1 X n term2).
 Proof.
-unfold subseqWrap0.
-destruct (natDiff n m) as [[i []] | [i []]];
- induction i; cbn; auto with parametricity.
+induction n; simpl; auto with parametricity.
 Qed.
-Hint Immediate subseqWrap0_Parametric : parametricity.
+Hint Resolve full_left_shift1_Parametric : parametricity.
 
-Lemma subseqWrapPair_Parametric {n m} z {term1 term2 : Core.Algebra} rec1 rec2 (R : Core.Parametric.Rel term1 term2) :
-  (forall m z, R (Word n) (Word m) (rec1 m z) (rec2 m z)) ->
-  R (Word n * Word n) (Word m) (subseqWrapPair z rec1) (subseqWrapPair z rec2).
+Lemma build_full_right_shift1_Parametric {term1 term2 : Core.Algebra} (R : Core.Parametric.Rel term1 term2)
+  {X W} t1 t2 : R (W * X) (X * W) t1 t2 -> R _ _ (build_full_right_shift1 t1) (build_full_right_shift1 t2).
 Proof.
-change (R (Word n * Word n)) with (R (Word (S n))).
-revert z; induction m; simpl subseqWrapPair; intros z Hrec;
-destruct (Z.eq_dec _ _) as [|];
-repeat (destruct Z_lt_le_dec);
-repeat first [apply pair_Parametric
-             |refine (drop_Parametric _ _ _ _)
-             |refine (take_Parametric _ _ _ _)];
-auto with parametricity.
+unfold build_full_right_shift1.
+auto 10 with parametricity.
 Qed.
-Hint Resolve subseqWrapPair_Parametric : parametricity.
+Hint Resolve build_full_right_shift1_Parametric : parametricity.
 
-Lemma subseqWrap_Parametric {n m} z {term1 term2 : Core.Algebra} (R : Core.Parametric.Rel term1 term2) :
-  R (Word n) (Word m) (subseqWrap z) (subseqWrap z).
+Lemma full_right_shift1_Parametric {term1 term2 : Core.Algebra} (R : Core.Parametric.Rel term1 term2)
+  {X n} : R _ _ full_right_shift1 (@full_right_shift1 X n term2).
 Proof.
-revert m z; induction n; simpl subseqWrap; auto with parametricity.
-simpl; auto with parametricity.
+induction n; simpl; auto with parametricity.
 Qed.
-Hint Immediate subseqWrap_Parametric : parametricity.
+Hint Resolve full_right_shift1_Parametric : parametricity.
 
-Lemma rotate_Parametric {n} z {term1 term2 : Core.Algebra} (R : Core.Parametric.Rel term1 term2) :
-  R (Word n) (Word n) (rotate z) (rotate z).
+Lemma left_shift1_Parametric {term1 term2 : Core.Algebra} (R : Core.Parametric.Rel term1 term2)
+  {X n} t1 t2 : R _ _ t1 t2 -> R _ _ (left_shift1 t1) (@left_shift1 X n term2 t2).
 Proof.
-unfold rotate.
-auto with parametricity.
+unfold left_shift1.
+auto 10 with parametricity.
 Qed.
-Hint Immediate rotate_Parametric : parametricity.
+Hint Resolve left_shift1_Parametric : parametricity.
+
+Lemma left_shift_const_by_Parametric {term1 term2 : Core.Algebra} (R : Core.Parametric.Rel term1 term2)
+  {X n} t1 t2 p : R _ _ t1 t2 -> R _ _ (left_shift_const_by t1 p) (@left_shift_const_by X n term2 t2 p).
+Proof.
+revert X t1 t2 p.
+induction n; intros X t1 t2 p Ht; simpl; destruct (_ <=? _)%Z; auto with parametricity.
+change (Vector X n * Vector X n) with (Vector X (S n)).
+destruct p;
+try apply comp_Parametric;auto 10 with parametricity;
+destruct (@eq_sym Ty (Vector X (S n)) (Vector (X * X) n) (@VectorPromote X n));
+apply IHn;auto 10 with parametricity.
+Qed.
+Hint Resolve left_shift_const_by_Parametric : parametricity.
+
+Lemma right_shift1_Parametric {term1 term2 : Core.Algebra} (R : Core.Parametric.Rel term1 term2)
+  {X n} t1 t2 : R _ _ t1 t2 -> R _ _ (right_shift1 t1) (@right_shift1 X n term2 t2).
+Proof.
+unfold right_shift1.
+auto 10 with parametricity.
+Qed.
+Hint Resolve right_shift1_Parametric : parametricity.
+
+Lemma right_shift_const_by_Parametric {term1 term2 : Core.Algebra} (R : Core.Parametric.Rel term1 term2)
+  {X n} t1 t2 p : R _ _ t1 t2 -> R _ _ (right_shift_const_by t1 p) (@right_shift_const_by X n term2 t2 p).
+Proof.
+revert X t1 t2 p.
+induction n; intros X t1 t2 p Ht; simpl; destruct (_ <=? _)%Z; auto with parametricity.
+change (Vector X n * Vector X n) with (Vector X (S n)).
+destruct p;
+try apply comp_Parametric;auto 10 with parametricity;
+destruct (@eq_sym Ty (Vector X (S n)) (Vector (X * X) n) (@VectorPromote X n));
+apply IHn;auto 10 with parametricity.
+Qed.
+Hint Resolve right_shift_const_by_Parametric : parametricity.
+
+Lemma shift_const_by_Parametric {term1 term2 : Core.Algebra} (R : Core.Parametric.Rel term1 term2)
+  {X n} t1 t2 z : R _ _ t1 t2 -> R _ _ (shift_const_by t1 z) (@shift_const_by X n term2 t2 z).
+Proof.
+destruct z;simpl;auto 10 with parametricity.
+Qed.
+Hint Resolve shift_const_by_Parametric : parametricity.
+
+Lemma shift_const_Parametric {n} z {term1 term2 : Core.Algebra} (R : Core.Parametric.Rel term1 term2) :
+  R (Word n) (Word n) (shift_const z) (shift_const z).
+Proof.
+unfold shift_const.
+apply shift_const_by_Parametric.
+auto 10 with parametricity.
+Qed.
+Hint Immediate shift_const_Parametric : parametricity.
+
+Lemma left_rotate1_Parametric {term1 term2 : Core.Algebra} (R : Core.Parametric.Rel term1 term2)
+  {X n} : R _ _ left_rotate1 (@left_rotate1 X n term2).
+Proof.
+unfold left_rotate1.
+auto 10 with parametricity.
+Qed.
+Hint Resolve left_rotate1_Parametric : parametricity.
+
+Lemma right_rotate1_Parametric {term1 term2 : Core.Algebra} (R : Core.Parametric.Rel term1 term2)
+  {X n} : R _ _ right_rotate1 (@right_rotate1 X n term2).
+Proof.
+unfold right_rotate1.
+auto 10 with parametricity.
+Qed.
+Hint Resolve right_rotate1_Parametric : parametricity.
+
+Lemma rotate_const_list_length {term1 term2 : Core.Algebra}
+  {X n} z : length (@rotate_const_list X n term1 z) = length (@rotate_const_list X n term2 z).
+Proof.
+revert X z.
+induction n; intros X z; simpl.
+- reflexivity.
+- repeat destruct (Z.even _);simpl;change (Vector X n * Vector X n) with (Vector X (S n));
+  destruct (@eq_sym Ty (Vector X (S n)) (Vector (X * X) n) (@VectorPromote X n)); simpl;
+  firstorder.
+Qed.
+
+Lemma rotate_const_list_Parametric {term1 term2 : Core.Algebra} (R : Core.Parametric.Rel term1 term2)
+  {X n} z i : R _ _ (nth i (@rotate_const_list X n term1 z) iden) (nth i (@rotate_const_list X n term2 z) iden).
+Proof.
+revert X z i.
+induction n; intros X z i; simpl.
+- destruct i; auto with parametricity.
+- repeat destruct (Z.even _);[|destruct i|destruct i];simpl;change (Vector X n * Vector X n) with (Vector X (S n));auto 10 with parametricity;
+  destruct (@eq_sym Ty (Vector X (S n)) (Vector (X * X) n) (@VectorPromote X n));apply IHn.
+Qed.
+
+Lemma foldr_comp_Parametric {term1 term2 : Core.Algebra} (R : Core.Parametric.Rel term1 term2)
+  {X} l1 l2 : length l1 = length l2 -> (forall i, R X X (nth i l1 iden) (nth i l2 iden)) -> R _ _ (foldr_comp l1) (foldr_comp l2).
+Proof.
+revert l2.
+induction l1; intros [|x l2]; simpl; try discriminate.
+- auto with parametricity.
+- intros H.
+  inversion H.
+  intros H0.
+  assert (H00 := H0 0).
+  destruct l1; destruct l2; try discriminate.
+  + assumption.
+  + apply comp_Parametric;[assumption|].
+    apply IHl1;[assumption|].
+    intros i.
+    apply (H0 (S i)).
+Qed.
+
+Lemma rotate_const_Parametric {n} z {term1 term2 : Core.Algebra} (R : Core.Parametric.Rel term1 term2) :
+  R (Word n) (Word n) (rotate_const z) (rotate_const z).
+Proof.
+unfold rotate_const.
+apply foldr_comp_Parametric.
+- apply rotate_const_list_length.
+- apply rotate_const_list_Parametric.
+Qed.
+Hint Immediate rotate_const_Parametric : parametricity.
